<?xml version="1.0"?>
<rdf:RDF xmlns="http://www.semanticweb.org/mguen/ontologies/2024/1/CognitiveBiasOntology/continued_influence_effect#"
     xml:base="http://www.semanticweb.org/mguen/ontologies/2024/1/CognitiveBiasOntology/continued_influence_effect"
     xmlns:ec="http://krisnadhi.github.io/onto/event.owl"
     xmlns:fs="http://etna.istc.cnr.it/framester2/data/framestercore/"
     xmlns:tp="http://ontologydesignpatterns.org/cp/owl/topic.owl"
     xmlns:acf="http://www.ontologydesignpatterns.org/ont/dul/DUL.owl"
     xmlns:cbo="http://www.semanticweb.org/mguen/ontologies/2024/1/CognitiveBiasOntology/continued_influence_effect"
     xmlns:owl="http://www.w3.org/2002/07/owl#"
     xmlns:rdf="http://www.w3.org/1999/02/22-rdf-syntax-ns#"
     xmlns:xml="http://www.w3.org/XML/1998/namespace"
     xmlns:xsd="http://www.w3.org/2001/XMLSchema#"
     xmlns:rdfs="http://www.w3.org/2000/01/rdf-schema#"
     xmlns:event="http://krisnadhi.github.io/onto/event.owl#"
     xmlns:terms="http://purl.org/dc/terms/"
     xmlns:topic="http://ontologydesignpatterns.org/cp/owl/topic.owl#"
     xmlns:continued_influence_effect="http://www.semanticweb.org/mguen/ontologies/2024/1/CognitiveBiasOntology/continued_influence_effect#">
    <owl:Ontology rdf:about="http://www.semanticweb.org/mguen/ontologies/2024/1/CognitiveBiasOntology/continued_influence_effect">
        <terms:created>15-02-2024</terms:created>
        <terms:creator>Matteo Guenci</terms:creator>
        <terms:description>The Continued Influence Effect section of the Cognitive Bias Ontology.</terms:description>
        <terms:title>The Continued Influence Effect Ontology</terms:title>
        <has_component>http://etna.istc.cnr.it/framester2/data/framestercore/</has_component>
        <has_component>http://krisnadhi.github.io/onto/event.owl</has_component>
        <has_component>http://ontologydesignpatterns.org/cp/owl/topic.owl</has_component>
        <has_component>http://www.ontologydesignpatterns.org/ont/dul/DUL.owl</has_component>
        <user_story>Meet John, a middle-aged man who grew up during the height of the space race. He&apos;s always been fascinated by space exploration, but he stumbled upon a documentary that claimed the moon landing was a hoax. The documentary presented various arguments, such as the waving flag and the absence of stars in the photos, which led John to question the authenticity of the moon landing.

Despite his doubts, John decided to do his own research. He read numerous articles and watched interviews with astronauts and scientists. Each source debunked the hoax claims and provided logical explanations for the arguments presented in the documentary. For example, the flag appeared to wave due to the way it was planted and the lack of air resistance on the moon, and the stars weren&apos;t visible in the photos due to the camera settings used.

However, even after learning the facts, John found himself still influenced by the documentary. Every time he thought about the moon landing, the hoax claims would resurface in his mind, casting a shadow of doubt. This is an example of the Continued Influence Effect. Despite being corrected, the misinformation continued to influence John&apos;s belief about the moon landing.

Eventually, John realized that he needed to actively remind himself of the facts whenever the hoax claims came to mind. Over time, he was able to reduce the influence of the misinformation, but it was a clear demonstration of how powerful the Continued Influence Effect can be.</user_story>
        <rdfs:comment>The Continued Influence Effect (CIE) is a psychological phenomenon referring to the tendency for misinformation to continue influencing peopleâ€™s thinking and decision-making even after it has been corrected or debunked. This effect occurs when individuals maintain their belief in false information, and it continues to shape their understanding and interpretation of related topics, despite being exposed to factual corrections.</rdfs:comment>
    </owl:Ontology>
    


    <!-- 
    ///////////////////////////////////////////////////////////////////////////////////////
    //
    // Annotation properties
    //
    ///////////////////////////////////////////////////////////////////////////////////////
     -->

    


    <!-- http://purl.org/dc/terms/created -->

    <owl:AnnotationProperty rdf:about="http://purl.org/dc/terms/created"/>
    


    <!-- http://purl.org/dc/terms/creator -->

    <owl:AnnotationProperty rdf:about="http://purl.org/dc/terms/creator"/>
    


    <!-- http://purl.org/dc/terms/description -->

    <owl:AnnotationProperty rdf:about="http://purl.org/dc/terms/description"/>
    


    <!-- http://purl.org/dc/terms/title -->

    <owl:AnnotationProperty rdf:about="http://purl.org/dc/terms/title"/>
    


    <!-- http://www.semanticweb.org/mguen/ontologies/2024/1/CognitiveBiasOntology/continued_influence_effect#has_component -->

    <owl:AnnotationProperty rdf:about="http://www.semanticweb.org/mguen/ontologies/2024/1/CognitiveBiasOntology/continued_influence_effect#has_component"/>
    


    <!-- http://www.semanticweb.org/mguen/ontologies/2024/1/CognitiveBiasOntology/continued_influence_effect#user_story -->

    <owl:AnnotationProperty rdf:about="http://www.semanticweb.org/mguen/ontologies/2024/1/CognitiveBiasOntology/continued_influence_effect#user_story"/>
    


    <!-- 
    ///////////////////////////////////////////////////////////////////////////////////////
    //
    // Object Properties
    //
    ///////////////////////////////////////////////////////////////////////////////////////
     -->

    


    <!-- http://etna.istc.cnr.it/framester2/data/framestercore/Research -->

    <owl:ObjectProperty rdf:about="http://etna.istc.cnr.it/framester2/data/framestercore/Research">
        <rdfs:domain rdf:resource="http://www.ontologydesignpatterns.org/ont/dul/DUL.owl#SocialAgent"/>
        <rdfs:range rdf:resource="http://www.semanticweb.org/mguen/ontologies/2024/1/CognitiveBiasOntology/continued_influence_effect#Source"/>
    </owl:ObjectProperty>
    


    <!-- http://krisnadhi.github.io/onto/event.owl#hasInformationObject -->

    <owl:ObjectProperty rdf:about="http://krisnadhi.github.io/onto/event.owl#hasInformationObject">
        <rdfs:domain rdf:resource="http://www.ontologydesignpatterns.org/ont/dul/DUL.owl#SocialAgent"/>
        <rdfs:range rdf:resource="http://etna.istc.cnr.it/framester2/data/framestercore/Information"/>
        <rdfs:comment>Property relating Event to InformationObject in this pattern. The domain of this property is not restricted to Event since it is possible that non-event to have an information object. The range is always InformationObject since it makes no sense to have a property named hasInformationObject to point to anything other than information object.</rdfs:comment>
    </owl:ObjectProperty>
    


    <!-- http://ontologydesignpatterns.org/cp/owl/topic.owl#hasTopic -->

    <owl:ObjectProperty rdf:about="http://ontologydesignpatterns.org/cp/owl/topic.owl#hasTopic">
        <rdfs:domain rdf:resource="http://etna.istc.cnr.it/framester2/data/framestercore/Information"/>
        <rdfs:range rdf:resource="http://ontologydesignpatterns.org/cp/owl/topic.owl#Topic"/>
        <rdfs:comment>(owl:ObjectProperty) The relation between something and its Topic (subject, argument, domain, theme, subject area, etc.). It can be used widely to talk about document annotations, subject directories, etc.</rdfs:comment>
        <rdfs:comment>Links misinformation or correction to the topic it pertains to</rdfs:comment>
    </owl:ObjectProperty>
    


    <!-- http://www.semanticweb.org/mguen/ontologies/2024/1/CognitiveBiasOntology/continued_influence_effect#keepInfluencing -->

    <owl:ObjectProperty rdf:about="http://www.semanticweb.org/mguen/ontologies/2024/1/CognitiveBiasOntology/continued_influence_effect#keepInfluencing">
        <rdfs:domain rdf:resource="http://etna.istc.cnr.it/framester2/data/framestercore/Information"/>
        <rdfs:range rdf:resource="http://www.ontologydesignpatterns.org/ont/dul/DUL.owl#SocialAgent"/>
        <rdfs:comment>links the Misinformation class to the SocialAgent, it represent the prolungated influence the Misinformation has on the SocialAgent</rdfs:comment>
    </owl:ObjectProperty>
    


    <!-- http://www.semanticweb.org/mguen/ontologies/2024/1/CognitiveBiasOntology/continued_influence_effect#originatesFrom -->

    <owl:ObjectProperty rdf:about="http://www.semanticweb.org/mguen/ontologies/2024/1/CognitiveBiasOntology/continued_influence_effect#originatesFrom">
        <rdfs:domain rdf:resource="http://etna.istc.cnr.it/framester2/data/framestercore/Information"/>
        <rdfs:range rdf:resource="http://www.semanticweb.org/mguen/ontologies/2024/1/CognitiveBiasOntology/continued_influence_effect#Source"/>
        <rdfs:comment>Links any piece of information to the source it originates from</rdfs:comment>
    </owl:ObjectProperty>
    


    <!-- 
    ///////////////////////////////////////////////////////////////////////////////////////
    //
    // Data properties
    //
    ///////////////////////////////////////////////////////////////////////////////////////
     -->

    


    <!-- http://www.semanticweb.org/mguen/ontologies/2024/1/CognitiveBiasOntology/continued_influence_effect#isCorrect -->

    <owl:DatatypeProperty rdf:about="http://www.semanticweb.org/mguen/ontologies/2024/1/CognitiveBiasOntology/continued_influence_effect#isCorrect">
        <rdfs:domain>
            <owl:Class>
                <owl:unionOf rdf:parseType="Collection">
                    <rdf:Description rdf:about="http://etna.istc.cnr.it/framester2/data/framestercore/Information"/>
                    <rdf:Description rdf:about="http://www.semanticweb.org/mguen/ontologies/2024/1/CognitiveBiasOntology/continued_influence_effect#Source"/>
                </owl:unionOf>
            </owl:Class>
        </rdfs:domain>
        <rdfs:range rdf:resource="http://www.w3.org/2001/XMLSchema#boolean"/>
        <rdfs:comment>a data property that states if the information or the source it originates from is valid or correct</rdfs:comment>
    </owl:DatatypeProperty>
    


    <!-- http://www.semanticweb.org/mguen/ontologies/2024/1/CognitiveBiasOntology/continued_influence_effect#isInfluenced -->

    <owl:DatatypeProperty rdf:about="http://www.semanticweb.org/mguen/ontologies/2024/1/CognitiveBiasOntology/continued_influence_effect#isInfluenced">
        <rdfs:domain rdf:resource="http://www.ontologydesignpatterns.org/ont/dul/DUL.owl#SocialAgent"/>
        <rdfs:range rdf:resource="http://www.w3.org/2001/XMLSchema#boolean"/>
        <rdfs:comment>a data property that states if the SocialAgent is influenced by information</rdfs:comment>
    </owl:DatatypeProperty>
    


    <!-- 
    ///////////////////////////////////////////////////////////////////////////////////////
    //
    // Classes
    //
    ///////////////////////////////////////////////////////////////////////////////////////
     -->

    


    <!-- http://etna.istc.cnr.it/framester2/data/framestercore/Information -->

    <owl:Class rdf:about="http://etna.istc.cnr.it/framester2/data/framestercore/Information">
        <owl:equivalentClass>
            <owl:Class>
                <owl:intersectionOf rdf:parseType="Collection">
                    <rdf:Description rdf:about="http://etna.istc.cnr.it/framester2/data/framestercore/Information"/>
                    <owl:Restriction>
                        <owl:onProperty rdf:resource="http://www.semanticweb.org/mguen/ontologies/2024/1/CognitiveBiasOntology/continued_influence_effect#originatesFrom"/>
                        <owl:someValuesFrom>
                            <owl:Class>
                                <owl:intersectionOf rdf:parseType="Collection">
                                    <rdf:Description rdf:about="http://www.semanticweb.org/mguen/ontologies/2024/1/CognitiveBiasOntology/continued_influence_effect#Source"/>
                                    <owl:Restriction>
                                        <owl:onProperty rdf:resource="http://www.semanticweb.org/mguen/ontologies/2024/1/CognitiveBiasOntology/continued_influence_effect#isCorrect"/>
                                        <owl:hasValue rdf:datatype="http://www.w3.org/2001/XMLSchema#boolean">false</owl:hasValue>
                                    </owl:Restriction>
                                </owl:intersectionOf>
                            </owl:Class>
                        </owl:someValuesFrom>
                    </owl:Restriction>
                    <owl:Restriction>
                        <owl:onProperty rdf:resource="http://www.semanticweb.org/mguen/ontologies/2024/1/CognitiveBiasOntology/continued_influence_effect#isCorrect"/>
                        <owl:hasValue rdf:datatype="http://www.w3.org/2001/XMLSchema#boolean">false</owl:hasValue>
                    </owl:Restriction>
                </owl:intersectionOf>
            </owl:Class>
        </owl:equivalentClass>
        <rdfs:subClassOf rdf:resource="http://krisnadhi.github.io/onto/event.owl#InformationObject"/>
        <rdfs:comment>A Cognizer knows or comes to know some piece of Information about a Topic. In this frame, many LUs encode a specific Means_of_Gathering and/or Source, but these may also be expressed separately. Also, the big problem is that our intel about WMD&apos;s has many times been wrong. Anyone got the straight dope on this? Get the inside scoop on sprint football player Austin Wilson. CNI I know him pretty well and I have a lot of dirt on him so I can always hold him over a barrel. What&apos;s the info about the new scanner chip? INI</rdfs:comment>
        <rdfs:comment>This expression represents an Information that has isCorrect value false and originates from a Source where isCorrect is also false. This means that if an Information has the isCorrect value set to false, then the Source it originates from also has the isCorrect value set to false.</rdfs:comment>
    </owl:Class>
    


    <!-- http://krisnadhi.github.io/onto/event.owl#InformationObject -->

    <owl:Class rdf:about="http://krisnadhi.github.io/onto/event.owl#InformationObject">
        <rdfs:comment>An entity that encapsulates all descriptive or non-defining information of the corresponding event, e.g., names, additional identifiers, textual descriptions, etc. Should normally be aligned to a separate Information Object pattern</rdfs:comment>
    </owl:Class>
    


    <!-- http://ontologydesignpatterns.org/cp/owl/topic.owl#Topic -->

    <owl:Class rdf:about="http://ontologydesignpatterns.org/cp/owl/topic.owl#Topic">
        <rdfs:comment>(owl:Class) A topic, or subject, argument, domain, theme, subject area, etc.</rdfs:comment>
        <rdfs:comment>Represents the subject matter of the information.</rdfs:comment>
    </owl:Class>
    


    <!-- http://www.ontologydesignpatterns.org/ont/dul/DUL.owl#SocialAgent -->

    <owl:Class rdf:about="http://www.ontologydesignpatterns.org/ont/dul/DUL.owl#SocialAgent">
        <owl:equivalentClass>
            <owl:Class>
                <owl:intersectionOf rdf:parseType="Collection">
                    <rdf:Description rdf:about="http://www.ontologydesignpatterns.org/ont/dul/DUL.owl#SocialAgent"/>
                    <owl:Restriction>
                        <owl:onProperty rdf:resource="http://www.semanticweb.org/mguen/ontologies/2024/1/CognitiveBiasOntology/continued_influence_effect#keepInfluencing"/>
                        <owl:someValuesFrom>
                            <owl:Class>
                                <owl:intersectionOf rdf:parseType="Collection">
                                    <rdf:Description rdf:about="http://etna.istc.cnr.it/framester2/data/framestercore/Information"/>
                                    <owl:Restriction>
                                        <owl:onProperty rdf:resource="http://www.semanticweb.org/mguen/ontologies/2024/1/CognitiveBiasOntology/continued_influence_effect#isCorrect"/>
                                        <owl:hasValue rdf:datatype="http://www.w3.org/2001/XMLSchema#boolean">false</owl:hasValue>
                                    </owl:Restriction>
                                </owl:intersectionOf>
                            </owl:Class>
                        </owl:someValuesFrom>
                    </owl:Restriction>
                    <owl:Restriction>
                        <owl:onProperty rdf:resource="http://www.semanticweb.org/mguen/ontologies/2024/1/CognitiveBiasOntology/continued_influence_effect#isInfluenced"/>
                        <owl:hasValue rdf:datatype="http://www.w3.org/2001/XMLSchema#boolean">true</owl:hasValue>
                    </owl:Restriction>
                </owl:intersectionOf>
            </owl:Class>
        </owl:equivalentClass>
        <rdfs:comment>(owl:Class) Any individual whose existence is granted simply by its social communicability and capability of action (through some PhysicalAgent)</rdfs:comment>
        <rdfs:comment>the &quot;equivalent to&quot; statement describes an anonymous class of SocialAgent instances that satisfy all of the following conditions:

The isInfluenced data property has a value of true.
They are related through the keepInfluencing object property to some instance of Information where the isCorrect data property has a value of false.
In other words: a SocialAgent that is influenced (isInfluenced value true) by some Information where isCorrect is false.</rdfs:comment>
    </owl:Class>
    


    <!-- http://www.semanticweb.org/mguen/ontologies/2024/1/CognitiveBiasOntology/continued_influence_effect#Source -->

    <owl:Class rdf:about="http://www.semanticweb.org/mguen/ontologies/2024/1/CognitiveBiasOntology/continued_influence_effect#Source">
        <rdfs:comment>Represents the origin of the information (e.g., media, word of mouth, etc.).</rdfs:comment>
    </owl:Class>
    


    <!-- 
    ///////////////////////////////////////////////////////////////////////////////////////
    //
    // Individuals
    //
    ///////////////////////////////////////////////////////////////////////////////////////
     -->

    


    <!-- http://etna.istc.cnr.it/framester2/data/framestercore/Research -->

    <owl:NamedIndividual rdf:about="http://etna.istc.cnr.it/framester2/data/framestercore/Research">
        <rdf:type rdf:resource="http://www.semanticweb.org/mguen/ontologies/2024/1/CognitiveBiasOntology/continued_influence_effect#Source"/>
        <owl:differentFrom rdf:resource="http://www.semanticweb.org/mguen/ontologies/2024/1/CognitiveBiasOntology/continued_influence_effect#Documentary"/>
        <isCorrect rdf:datatype="http://www.w3.org/2001/XMLSchema#boolean">true</isCorrect>
    </owl:NamedIndividual>
    


    <!-- http://www.semanticweb.org/mguen/ontologies/2024/1/CognitiveBiasOntology/continued_influence_effect#AbsenceOfStars -->

    <owl:NamedIndividual rdf:about="http://www.semanticweb.org/mguen/ontologies/2024/1/CognitiveBiasOntology/continued_influence_effect#AbsenceOfStars">
        <rdf:type rdf:resource="http://etna.istc.cnr.it/framester2/data/framestercore/Information"/>
        <topic:hasTopic rdf:resource="http://www.semanticweb.org/mguen/ontologies/2024/1/CognitiveBiasOntology/continued_influence_effect#SpaceExploration"/>
        <keepInfluencing rdf:resource="http://www.semanticweb.org/mguen/ontologies/2024/1/CognitiveBiasOntology/continued_influence_effect#John"/>
        <originatesFrom rdf:resource="http://www.semanticweb.org/mguen/ontologies/2024/1/CognitiveBiasOntology/continued_influence_effect#Documentary"/>
        <rdfs:comment>the first encounter with this evidence in the documentary</rdfs:comment>
    </owl:NamedIndividual>
    


    <!-- http://www.semanticweb.org/mguen/ontologies/2024/1/CognitiveBiasOntology/continued_influence_effect#AbsenceOfStars1 -->

    <owl:NamedIndividual rdf:about="http://www.semanticweb.org/mguen/ontologies/2024/1/CognitiveBiasOntology/continued_influence_effect#AbsenceOfStars1">
        <rdf:type rdf:resource="http://etna.istc.cnr.it/framester2/data/framestercore/Information"/>
        <topic:hasTopic rdf:resource="http://www.semanticweb.org/mguen/ontologies/2024/1/CognitiveBiasOntology/continued_influence_effect#SpaceExploration"/>
        <originatesFrom rdf:resource="http://etna.istc.cnr.it/framester2/data/framestercore/Research"/>
    </owl:NamedIndividual>
    


    <!-- http://www.semanticweb.org/mguen/ontologies/2024/1/CognitiveBiasOntology/continued_influence_effect#Documentary -->

    <owl:NamedIndividual rdf:about="http://www.semanticweb.org/mguen/ontologies/2024/1/CognitiveBiasOntology/continued_influence_effect#Documentary">
        <rdf:type rdf:resource="http://www.semanticweb.org/mguen/ontologies/2024/1/CognitiveBiasOntology/continued_influence_effect#Source"/>
        <isCorrect rdf:datatype="http://www.w3.org/2001/XMLSchema#boolean">false</isCorrect>
    </owl:NamedIndividual>
    


    <!-- http://www.semanticweb.org/mguen/ontologies/2024/1/CognitiveBiasOntology/continued_influence_effect#John -->

    <owl:NamedIndividual rdf:about="http://www.semanticweb.org/mguen/ontologies/2024/1/CognitiveBiasOntology/continued_influence_effect#John">
        <rdf:type rdf:resource="http://www.ontologydesignpatterns.org/ont/dul/DUL.owl#SocialAgent"/>
        <fs:Research rdf:resource="http://etna.istc.cnr.it/framester2/data/framestercore/Research"/>
        <fs:Research rdf:resource="http://www.semanticweb.org/mguen/ontologies/2024/1/CognitiveBiasOntology/continued_influence_effect#Documentary"/>
        <event:hasInformationObject rdf:resource="http://www.semanticweb.org/mguen/ontologies/2024/1/CognitiveBiasOntology/continued_influence_effect#AbsenceOfStars"/>
        <event:hasInformationObject rdf:resource="http://www.semanticweb.org/mguen/ontologies/2024/1/CognitiveBiasOntology/continued_influence_effect#AbsenceOfStars1"/>
        <event:hasInformationObject rdf:resource="http://www.semanticweb.org/mguen/ontologies/2024/1/CognitiveBiasOntology/continued_influence_effect#WawingFlag"/>
        <event:hasInformationObject rdf:resource="http://www.semanticweb.org/mguen/ontologies/2024/1/CognitiveBiasOntology/continued_influence_effect#WawingFlag1"/>
        <isInfluenced>true or false</isInfluenced>
    </owl:NamedIndividual>
    


    <!-- http://www.semanticweb.org/mguen/ontologies/2024/1/CognitiveBiasOntology/continued_influence_effect#SpaceExploration -->

    <owl:NamedIndividual rdf:about="http://www.semanticweb.org/mguen/ontologies/2024/1/CognitiveBiasOntology/continued_influence_effect#SpaceExploration">
        <rdf:type rdf:resource="http://ontologydesignpatterns.org/cp/owl/topic.owl#Topic"/>
    </owl:NamedIndividual>
    


    <!-- http://www.semanticweb.org/mguen/ontologies/2024/1/CognitiveBiasOntology/continued_influence_effect#WawingFlag -->

    <owl:NamedIndividual rdf:about="http://www.semanticweb.org/mguen/ontologies/2024/1/CognitiveBiasOntology/continued_influence_effect#WawingFlag">
        <rdf:type rdf:resource="http://etna.istc.cnr.it/framester2/data/framestercore/Information"/>
        <topic:hasTopic rdf:resource="http://www.semanticweb.org/mguen/ontologies/2024/1/CognitiveBiasOntology/continued_influence_effect#SpaceExploration"/>
        <keepInfluencing rdf:resource="http://www.semanticweb.org/mguen/ontologies/2024/1/CognitiveBiasOntology/continued_influence_effect#John"/>
        <originatesFrom rdf:resource="http://www.semanticweb.org/mguen/ontologies/2024/1/CognitiveBiasOntology/continued_influence_effect#Documentary"/>
    </owl:NamedIndividual>
    


    <!-- http://www.semanticweb.org/mguen/ontologies/2024/1/CognitiveBiasOntology/continued_influence_effect#WawingFlag1 -->

    <owl:NamedIndividual rdf:about="http://www.semanticweb.org/mguen/ontologies/2024/1/CognitiveBiasOntology/continued_influence_effect#WawingFlag1">
        <rdf:type rdf:resource="http://etna.istc.cnr.it/framester2/data/framestercore/Information"/>
        <topic:hasTopic rdf:resource="http://www.semanticweb.org/mguen/ontologies/2024/1/CognitiveBiasOntology/continued_influence_effect#SpaceExploration"/>
        <originatesFrom rdf:resource="http://etna.istc.cnr.it/framester2/data/framestercore/Research"/>
    </owl:NamedIndividual>
    


    <!-- 
    ///////////////////////////////////////////////////////////////////////////////////////
    //
    // Annotations
    //
    ///////////////////////////////////////////////////////////////////////////////////////
     -->

    <rdf:Description rdf:about="http://etna.istc.cnr.it/framester2/data/framestercore/Research">
        <rdfs:comment>A Researcher (an individual a group or institution) attempts to answer a Question by means of consulting literature, observation, or conducting experiments in a particular Field pertinent to the Question. The Question may be underspecified in the form of a Topic. Simmons and Nadel did research pertaining to Ardea purpurea and Egretta garzetta in 1998</rdfs:comment>
    </rdf:Description>
</rdf:RDF>



<!-- Generated by the OWL API (version 4.5.25.2023-02-15T19:15:49Z) https://github.com/owlcs/owlapi -->

