<?xml version="1.0"?>
<rdf:RDF xmlns="http://www.semanticweb.org/lucia/ontologies/2024/0/next-in-line#"
     xml:base="http://www.semanticweb.org/lucia/ontologies/2024/0/next-in-line"
     xmlns:cbo="http://www.semanticweb.org/lucia/ontologies/2024/0/CognitiveBiasOntology/next-in-line/"
     xmlns:owl="http://www.w3.org/2002/07/owl#"
     xmlns:rdf="http://www.w3.org/1999/02/22-rdf-syntax-ns#"
     xmlns:xml="http://www.w3.org/XML/1998/namespace"
     xmlns:xsd="http://www.w3.org/2001/XMLSchema#"
     xmlns:rdfs="http://www.w3.org/2000/01/rdf-schema#">
    <owl:Ontology rdf:about="http://www.semanticweb.org/lucia/ontologies/2024/0/next-in-line">
        <rdfs:comment>This is an ontology related to the cognitive bias effect &quot;next-in-line&quot;</rdfs:comment>
    </owl:Ontology>
    


    <!-- 
    ///////////////////////////////////////////////////////////////////////////////////////
    //
    // Object Properties
    //
    ///////////////////////////////////////////////////////////////////////////////////////
     -->

    


    <!-- http://www.semanticweb.org/lucia/ontologies/2024/0/next-in-line#contextOf -->

    <owl:ObjectProperty rdf:about="http://www.semanticweb.org/lucia/ontologies/2024/0/next-in-line#contextOf">
        <rdfs:domain rdf:resource="http://www.semanticweb.org/lucia/ontologies/2024/0/next-in-line#Turn"/>
        <rdfs:range rdf:resource="http://www.semanticweb.org/lucia/ontologies/2024/0/next-in-line#Discussion"/>
        <rdfs:comment>Links a Turn to the overarching Discussion, providing context for when it occurred</rdfs:comment>
    </owl:ObjectProperty>
    


    <!-- http://www.semanticweb.org/lucia/ontologies/2024/0/next-in-line#hasMemoryRecord -->

    <owl:ObjectProperty rdf:about="http://www.semanticweb.org/lucia/ontologies/2024/0/next-in-line#hasMemoryRecord">
        <rdfs:domain rdf:resource="http://www.semanticweb.org/lucia/ontologies/2024/0/next-in-line#Participant"/>
        <rdfs:range rdf:resource="http://www.semanticweb.org/lucia/ontologies/2024/0/next-in-line#Memory_Record"/>
        <rdfs:comment>Connects a Participant to their Memory Record, indicating what they remember from the discussion</rdfs:comment>
    </owl:ObjectProperty>
    


    <!-- http://www.semanticweb.org/lucia/ontologies/2024/0/next-in-line#hasParticipant -->

    <owl:ObjectProperty rdf:about="http://www.semanticweb.org/lucia/ontologies/2024/0/next-in-line#hasParticipant">
        <rdfs:domain rdf:resource="http://www.semanticweb.org/lucia/ontologies/2024/0/next-in-line#Discussion"/>
        <rdfs:range rdf:resource="http://www.semanticweb.org/lucia/ontologies/2024/0/next-in-line#Participant"/>
        <rdfs:comment>Describes the relationship between a Discussion and the Participants involved</rdfs:comment>
    </owl:ObjectProperty>
    


    <!-- http://www.semanticweb.org/lucia/ontologies/2024/0/next-in-line#hasTurn -->

    <owl:ObjectProperty rdf:about="http://www.semanticweb.org/lucia/ontologies/2024/0/next-in-line#hasTurn">
        <rdfs:domain rdf:resource="http://www.semanticweb.org/lucia/ontologies/2024/0/next-in-line#Participant"/>
        <rdfs:range rdf:resource="http://www.semanticweb.org/lucia/ontologies/2024/0/next-in-line#Turn"/>
        <rdfs:comment>Connects a Discussion to the sequence of Turns taken by the Participants</rdfs:comment>
    </owl:ObjectProperty>
    


    <!-- 
    ///////////////////////////////////////////////////////////////////////////////////////
    //
    // Classes
    //
    ///////////////////////////////////////////////////////////////////////////////////////
     -->

    


    <!-- http://www.semanticweb.org/lucia/ontologies/2024/0/next-in-line#Discussion -->

    <owl:Class rdf:about="http://www.semanticweb.org/lucia/ontologies/2024/0/next-in-line#Discussion">
        <rdfs:comment>Represents the overall context of a conversation where participants take turns</rdfs:comment>
    </owl:Class>
    


    <!-- http://www.semanticweb.org/lucia/ontologies/2024/0/next-in-line#Memory_Record -->

    <owl:Class rdf:about="http://www.semanticweb.org/lucia/ontologies/2024/0/next-in-line#Memory_Record">
        <rdfs:comment>Represents the memory of an individual regarding what was said during the conversation</rdfs:comment>
    </owl:Class>
    


    <!-- http://www.semanticweb.org/lucia/ontologies/2024/0/next-in-line#Participant -->

    <owl:Class rdf:about="http://www.semanticweb.org/lucia/ontologies/2024/0/next-in-line#Participant">
        <rdfs:comment>Represents an individual taking part in a discussion or conversation</rdfs:comment>
    </owl:Class>
    


    <!-- http://www.semanticweb.org/lucia/ontologies/2024/0/next-in-line#Turn -->

    <owl:Class rdf:about="http://www.semanticweb.org/lucia/ontologies/2024/0/next-in-line#Turn">
        <rdfs:comment>Represents a specific instance of an individual expressing their thoughts or ideas during a conversation</rdfs:comment>
    </owl:Class>
</rdf:RDF>



<!-- Generated by the OWL API (version 4.5.25.2023-02-15T19:15:49Z) https://github.com/owlcs/owlapi -->

