<?xml version="1.0"?>
<rdf:RDF xmlns="http://www.semanticweb.org/mguen/ontologies/2024/0/cognitive_bias_ontology_ostrich_effect#"
     xml:base="http://www.semanticweb.org/mguen/ontologies/2024/0/cognitive_bias_ontology_ostrich_effect"
     xmlns:cbo="http://www.semanticweb.org/mguen/ontologies/2024/0/cognitive_bias_ontology_ostrich_effect/"
     xmlns:owl="http://www.w3.org/2002/07/owl#"
     xmlns:rdf="http://www.w3.org/1999/02/22-rdf-syntax-ns#"
     xmlns:xml="http://www.w3.org/XML/1998/namespace"
     xmlns:xsd="http://www.w3.org/2001/XMLSchema#"
     xmlns:rdfs="http://www.w3.org/2000/01/rdf-schema#">
    <owl:Ontology rdf:about="http://www.semanticweb.org/mguen/ontologies/2024/0/cognitive_bias_ontology_ostrich_effect"/>
    


    <!-- 
    ///////////////////////////////////////////////////////////////////////////////////////
    //
    // Object Properties
    //
    ///////////////////////////////////////////////////////////////////////////////////////
     -->

    


    <!-- http://www.semanticweb.org/mguen/ontologies/2024/0/cognitive_bias_ontology_ostrich_effect#avoids -->

    <owl:ObjectProperty rdf:about="http://www.semanticweb.org/mguen/ontologies/2024/0/cognitive_bias_ontology_ostrich_effect#avoids">
        <rdfs:domain rdf:resource="http://www.semanticweb.org/mguen/ontologies/2024/0/cognitive_bias_ontology_ostrich_effect#Individual"/>
        <rdfs:range rdf:resource="http://www.semanticweb.org/mguen/ontologies/2024/0/cognitive_bias_ontology_ostrich_effect#NegativeInformation"/>
        <rdfs:comment>This property indicates that the individual is avoiding the negative information.</rdfs:comment>
    </owl:ObjectProperty>
    


    <!-- http://www.semanticweb.org/mguen/ontologies/2024/0/cognitive_bias_ontology_ostrich_effect#exhibitsIn -->

    <owl:ObjectProperty rdf:about="http://www.semanticweb.org/mguen/ontologies/2024/0/cognitive_bias_ontology_ostrich_effect#exhibitsIn">
        <rdfs:domain rdf:resource="http://www.semanticweb.org/mguen/ontologies/2024/0/cognitive_bias_ontology_ostrich_effect#Individual"/>
        <rdfs:range rdf:resource="http://www.semanticweb.org/mguen/ontologies/2024/0/cognitive_bias_ontology_ostrich_effect#Context"/>
        <rdfs:comment>This property shows the context in which the individual is exhibiting the Ostrich Effect.</rdfs:comment>
    </owl:ObjectProperty>
    


    <!-- http://www.semanticweb.org/mguen/ontologies/2024/0/cognitive_bias_ontology_ostrich_effect#feels -->

    <owl:ObjectProperty rdf:about="http://www.semanticweb.org/mguen/ontologies/2024/0/cognitive_bias_ontology_ostrich_effect#feels">
        <rdfs:domain rdf:resource="http://www.semanticweb.org/mguen/ontologies/2024/0/cognitive_bias_ontology_ostrich_effect#Individual"/>
        <rdfs:range rdf:resource="http://www.semanticweb.org/mguen/ontologies/2024/0/cognitive_bias_ontology_ostrich_effect#Emotion"/>
        <rdfs:comment>This property captures the emotions felt by the individual when faced with the negative information.</rdfs:comment>
    </owl:ObjectProperty>
    


    <!-- http://www.semanticweb.org/mguen/ontologies/2024/0/cognitive_bias_ontology_ostrich_effect#leadsTo -->

    <owl:ObjectProperty rdf:about="http://www.semanticweb.org/mguen/ontologies/2024/0/cognitive_bias_ontology_ostrich_effect#leadsTo">
        <rdfs:domain rdf:resource="http://www.semanticweb.org/mguen/ontologies/2024/0/cognitive_bias_ontology_ostrich_effect#OstrichEffect"/>
        <rdfs:range rdf:resource="http://www.semanticweb.org/mguen/ontologies/2024/0/cognitive_bias_ontology_ostrich_effect#Outcome"/>
        <rdfs:comment>This property shows the outcome of the individual&apos;s avoidance behavior.</rdfs:comment>
    </owl:ObjectProperty>
    


    <!-- http://www.semanticweb.org/mguen/ontologies/2024/0/cognitive_bias_ontology_ostrich_effect#occursIn -->

    <owl:ObjectProperty rdf:about="http://www.semanticweb.org/mguen/ontologies/2024/0/cognitive_bias_ontology_ostrich_effect#occursIn">
        <rdfs:domain rdf:resource="http://www.semanticweb.org/mguen/ontologies/2024/0/cognitive_bias_ontology_ostrich_effect#OstrichEffect"/>
        <rdfs:range rdf:resource="http://www.semanticweb.org/mguen/ontologies/2024/0/cognitive_bias_ontology_ostrich_effect#Context"/>
        <rdfs:comment>property that links instances of the OstrichEffect class to the Context in which they occur.</rdfs:comment>
    </owl:ObjectProperty>
    


    <!-- http://www.semanticweb.org/mguen/ontologies/2024/0/cognitive_bias_ontology_ostrich_effect#relatesTo -->

    <owl:ObjectProperty rdf:about="http://www.semanticweb.org/mguen/ontologies/2024/0/cognitive_bias_ontology_ostrich_effect#relatesTo">
        <rdfs:domain rdf:resource="http://www.semanticweb.org/mguen/ontologies/2024/0/cognitive_bias_ontology_ostrich_effect#NegativeInformation"/>
        <rdfs:range rdf:resource="http://www.semanticweb.org/mguen/ontologies/2024/0/cognitive_bias_ontology_ostrich_effect#Context"/>
        <rdfs:comment>This property links the negative information to the context in which it exists.</rdfs:comment>
    </owl:ObjectProperty>
    


    <!-- http://www.semanticweb.org/mguen/ontologies/2024/0/cognitive_bias_ontology_ostrich_effect#uses -->

    <owl:ObjectProperty rdf:about="http://www.semanticweb.org/mguen/ontologies/2024/0/cognitive_bias_ontology_ostrich_effect#uses">
        <rdfs:domain rdf:resource="http://www.semanticweb.org/mguen/ontologies/2024/0/cognitive_bias_ontology_ostrich_effect#Individual"/>
        <rdfs:range rdf:resource="http://www.semanticweb.org/mguen/ontologies/2024/0/cognitive_bias_ontology_ostrich_effect#CopingStrategy"/>
        <rdfs:comment>This property indicates the coping strategies used by the individual to deal with the negative information.</rdfs:comment>
    </owl:ObjectProperty>
    


    <!-- 
    ///////////////////////////////////////////////////////////////////////////////////////
    //
    // Classes
    //
    ///////////////////////////////////////////////////////////////////////////////////////
     -->

    


    <!-- http://www.semanticweb.org/mguen/ontologies/2024/0/cognitive_bias_ontology_ostrich_effect#Context -->

    <owl:Class rdf:about="http://www.semanticweb.org/mguen/ontologies/2024/0/cognitive_bias_ontology_ostrich_effect#Context">
        <rdfs:comment>The specific situation or domain in which the Ostrich Effect is being exhibited.</rdfs:comment>
    </owl:Class>
    


    <!-- http://www.semanticweb.org/mguen/ontologies/2024/0/cognitive_bias_ontology_ostrich_effect#CopingStrategy -->

    <owl:Class rdf:about="http://www.semanticweb.org/mguen/ontologies/2024/0/cognitive_bias_ontology_ostrich_effect#CopingStrategy">
        <rdfs:comment>The methods used by the individual to deal with the negative information.</rdfs:comment>
    </owl:Class>
    


    <!-- http://www.semanticweb.org/mguen/ontologies/2024/0/cognitive_bias_ontology_ostrich_effect#Emotion -->

    <owl:Class rdf:about="http://www.semanticweb.org/mguen/ontologies/2024/0/cognitive_bias_ontology_ostrich_effect#Emotion">
        <rdfs:comment>The feelings experienced by the individual when faced with the negative information.</rdfs:comment>
    </owl:Class>
    


    <!-- http://www.semanticweb.org/mguen/ontologies/2024/0/cognitive_bias_ontology_ostrich_effect#Individual -->

    <owl:Class rdf:about="http://www.semanticweb.org/mguen/ontologies/2024/0/cognitive_bias_ontology_ostrich_effect#Individual">
        <rdfs:comment>The person exhibiting the Ostrich Effect.</rdfs:comment>
    </owl:Class>
    


    <!-- http://www.semanticweb.org/mguen/ontologies/2024/0/cognitive_bias_ontology_ostrich_effect#NegativeInformation -->

    <owl:Class rdf:about="http://www.semanticweb.org/mguen/ontologies/2024/0/cognitive_bias_ontology_ostrich_effect#NegativeInformation">
        <rdfs:comment>The potentially distressing information that the individual is avoiding.</rdfs:comment>
    </owl:Class>
    


    <!-- http://www.semanticweb.org/mguen/ontologies/2024/0/cognitive_bias_ontology_ostrich_effect#OstrichEffect -->

    <owl:Class rdf:about="http://www.semanticweb.org/mguen/ontologies/2024/0/cognitive_bias_ontology_ostrich_effect#OstrichEffect">
        <rdfs:comment>Instances of the phenomenon where an individual avoids negative information.</rdfs:comment>
    </owl:Class>
    


    <!-- http://www.semanticweb.org/mguen/ontologies/2024/0/cognitive_bias_ontology_ostrich_effect#Outcome -->

    <owl:Class rdf:about="http://www.semanticweb.org/mguen/ontologies/2024/0/cognitive_bias_ontology_ostrich_effect#Outcome">
        <rdfs:comment>The result of the individual&apos;s avoidance behavior.</rdfs:comment>
    </owl:Class>
    


    <!-- 
    ///////////////////////////////////////////////////////////////////////////////////////
    //
    // Individuals
    //
    ///////////////////////////////////////////////////////////////////////////////////////
     -->

    


    <!-- http://www.semanticweb.org/mguen/ontologies/2024/0/cognitive_bias_ontology_ostrich_effect#AcademicSetting -->

    <owl:NamedIndividual rdf:about="http://www.semanticweb.org/mguen/ontologies/2024/0/cognitive_bias_ontology_ostrich_effect#AcademicSetting">
        <rdf:type rdf:resource="http://www.semanticweb.org/mguen/ontologies/2024/0/cognitive_bias_ontology_ostrich_effect#Context"/>
    </owl:NamedIndividual>
    


    <!-- http://www.semanticweb.org/mguen/ontologies/2024/0/cognitive_bias_ontology_ostrich_effect#Alex -->

    <owl:NamedIndividual rdf:about="http://www.semanticweb.org/mguen/ontologies/2024/0/cognitive_bias_ontology_ostrich_effect#Alex">
        <rdf:type rdf:resource="http://www.semanticweb.org/mguen/ontologies/2024/0/cognitive_bias_ontology_ostrich_effect#Individual"/>
    </owl:NamedIndividual>
    


    <!-- http://www.semanticweb.org/mguen/ontologies/2024/0/cognitive_bias_ontology_ostrich_effect#AvoidanceOfBadGrades -->

    <owl:NamedIndividual rdf:about="http://www.semanticweb.org/mguen/ontologies/2024/0/cognitive_bias_ontology_ostrich_effect#AvoidanceOfBadGrades">
        <rdf:type rdf:resource="http://www.semanticweb.org/mguen/ontologies/2024/0/cognitive_bias_ontology_ostrich_effect#OstrichEffect"/>
    </owl:NamedIndividual>
    


    <!-- http://www.semanticweb.org/mguen/ontologies/2024/0/cognitive_bias_ontology_ostrich_effect#PoorGrade -->

    <owl:NamedIndividual rdf:about="http://www.semanticweb.org/mguen/ontologies/2024/0/cognitive_bias_ontology_ostrich_effect#PoorGrade">
        <rdf:type rdf:resource="http://www.semanticweb.org/mguen/ontologies/2024/0/cognitive_bias_ontology_ostrich_effect#NegativeInformation"/>
    </owl:NamedIndividual>
</rdf:RDF>



<!-- Generated by the OWL API (version 4.5.25.2023-02-15T19:15:49Z) https://github.com/owlcs/owlapi -->

