<?xml version="1.0"?>
<rdf:RDF xmlns="http://www.semanticweb.org/mguen/ontologies/2024/0/CognitiveBiasOntology/ostrich_effect#"
     xml:base="http://www.semanticweb.org/mguen/ontologies/2024/0/CognitiveBiasOntology/ostrich_effect"
     xmlns:ac="http://www.ontology.se/odp/content/owl/Action.owl"
     xmlns:ec="http://krisnadhi.github.io/onto/event.owl"
     xmlns:en="http://etna.istc.cnr.it/framester2/conceptnet/5.7.0/c/en/"
     xmlns:fs="http://etna.istc.cnr.it/framester2/data/framestercore/"
     xmlns:st="http://www.ontologydesignpatterns.org/cp/owl/situation.owl"
     xmlns:acf="http://www.ontologydesignpatterns.org/ont/dul/DUL.owl"
     xmlns:cbo="http://www.semanticweb.org/mguen/ontologies/2024/0/cognitive_bias_ontology_ostrich_effect/"
     xmlns:owl="http://www.w3.org/2002/07/owl#"
     xmlns:rdf="http://www.w3.org/1999/02/22-rdf-syntax-ns#"
     xmlns:xml="http://www.w3.org/XML/1998/namespace"
     xmlns:xsd="http://www.w3.org/2001/XMLSchema#"
     xmlns:actp="http://descartes-core.org/ontologies/activities/1.0/ActivityPattern.owl"
     xmlns:foaf="http://xmlns.com/foaf/0.1/"
     xmlns:rdfs="http://www.w3.org/2000/01/rdf-schema#"
     xmlns:event="http://krisnadhi.github.io/onto/event.owl#"
     xmlns:Action="http://www.ontology.se/odp/content/owl/Action.owl#"
     xmlns:dcterms="http://purl.org/dc/terms/"
     xmlns:situation="http://www.ontologydesignpatterns.org/cp/owl/situation.owl#"
     xmlns:dbpedia-owl="https://en.wiktionary.org/wiki/"
     xmlns:ostrich_effect="http://www.semanticweb.org/mguen/ontologies/2024/0/CognitiveBiasOntology/ostrich_effect#"
     xmlns:ActivityPattern="http://descartes-core.org/ontologies/activities/1.0/ActivityPattern.owl#">
    <owl:Ontology rdf:about="http://www.semanticweb.org/mguen/ontologies/2024/0/CognitiveBiasOntology/ostrich_effect">
        <dcterms:created>5-02-2024</dcterms:created>
        <dcterms:creator>Matteo Guenci</dcterms:creator>
        <dcterms:description>The Ostrich effect section of the Cognitive Bias Ontology.</dcterms:description>
        <dcterms:title>Ostrich effect Ontology</dcterms:title>
        <hasComponent>http://descartes-core.org/ontologies/activities/1.0/ActivityPattern.owl</hasComponent>
        <hasComponent>http://krisnadhi.github.io/onto/event.owl</hasComponent>
        <hasComponent>http://ontologydesignpatterns.org/wiki/Submissions:Action</hasComponent>
        <hasComponent>http://www.ontologydesignpatterns.org/cp/owl/situation.owl</hasComponent>
        <hasComponent>http://www.ontologydesignpatterns.org/ont/dul/DUL.owl</hasComponent>
        <user_story>Meet Alex, a college student majoring in Computer Science. Alex has always been a diligent student, but the past semester was particularly challenging due to a heavy course load and personal issues. Despite his best efforts, he struggled with a few of his classes, especially Data Structures.

After the final exams, Alex found himself dreading the moment he would have to check his grades. He was particularly worried about his Data Structures grade. The fear of seeing a poor grade, and the negative emotions associated with it, led him to avoid checking his academic portal altogether. Days turned into weeks, and Alex still hadn&apos;t checked his grades.

This is an example of the Ostrich Effect. By avoiding potentially negative information, Alex was trying to escape the discomfort associated with it. However, this avoidance didn&apos;t change his academic situation and only added to his stress and anxiety.

Eventually, Alex realized that facing his fears was the only way forward. He finally checked his grades and, as expected, his score in Data Structures was lower than he&apos;d hoped. But now that he had confronted the reality, he was able to make a plan to improve his understanding of the subject and perform better in the future. By overcoming the Ostrich Effect, Alex took an important step towards academic growth and personal development.</user_story>
        <rdfs:comment>The Ostrich Effect, also known as the ostrich problem, is a cognitive bias where people tend to avoid potentially negative but useful information, such as feedback on progress, to avoid psychological discomfort1. This effect is named after the common (but false) legend that ostriches bury their heads in the sand to avoid danger1.

For example, in a financial context, people might avoid checking their bank account balance after spending a lot of money1. In healthcare, people with conditions like diabetes might avoid monitoring their blood sugar levels1. In the context of personal goals, someone aiming to lose weight might avoid weighing themselves or tracking their food intake2.

The term was originally coined by Galai &amp; Sade (2003), and there is neuroscientific evidence supporting the existence of this bias1. Itâ€™s important to be aware of the Ostrich Effect as it can lead to detrimental outcomes in various situations2.</rdfs:comment>
    </owl:Ontology>
    


    <!-- 
    ///////////////////////////////////////////////////////////////////////////////////////
    //
    // Annotation properties
    //
    ///////////////////////////////////////////////////////////////////////////////////////
     -->

    


    <!-- http://purl.org/dc/terms/created -->

    <owl:AnnotationProperty rdf:about="http://purl.org/dc/terms/created"/>
    


    <!-- http://purl.org/dc/terms/creator -->

    <owl:AnnotationProperty rdf:about="http://purl.org/dc/terms/creator"/>
    


    <!-- http://purl.org/dc/terms/description -->

    <owl:AnnotationProperty rdf:about="http://purl.org/dc/terms/description"/>
    


    <!-- http://purl.org/dc/terms/title -->

    <owl:AnnotationProperty rdf:about="http://purl.org/dc/terms/title"/>
    


    <!-- http://www.semanticweb.org/mguen/ontologies/2024/0/CognitiveBiasOntology/ostrich_effect#hasComponent -->

    <owl:AnnotationProperty rdf:about="http://www.semanticweb.org/mguen/ontologies/2024/0/CognitiveBiasOntology/ostrich_effect#hasComponent"/>
    


    <!-- http://www.semanticweb.org/mguen/ontologies/2024/0/CognitiveBiasOntology/ostrich_effect#user_story -->

    <owl:AnnotationProperty rdf:about="http://www.semanticweb.org/mguen/ontologies/2024/0/CognitiveBiasOntology/ostrich_effect#user_story"/>
    


    <!-- 
    ///////////////////////////////////////////////////////////////////////////////////////
    //
    // Object Properties
    //
    ///////////////////////////////////////////////////////////////////////////////////////
     -->

    


    <!-- http://descartes-core.org/ontologies/activities/1.0/ActivityPattern.owl#produces -->

    <owl:ObjectProperty rdf:about="http://descartes-core.org/ontologies/activities/1.0/ActivityPattern.owl#produces">
        <rdfs:domain rdf:resource="http://www.semanticweb.org/mguen/ontologies/2024/0/CognitiveBiasOntology/ostrich_effect#Behavior"/>
        <rdfs:range rdf:resource="http://descartes-core.org/ontologies/activities/1.0/ActivityPattern.owl#Outcome"/>
        <rdfs:comment>Link the behavior conducted by the SocialAgent to the Outcome</rdfs:comment>
    </owl:ObjectProperty>
    


    <!-- http://etna.istc.cnr.it/framester2/conceptnet/5.7.0/c/en/uses -->

    <owl:ObjectProperty rdf:about="http://etna.istc.cnr.it/framester2/conceptnet/5.7.0/c/en/uses">
        <rdfs:domain rdf:resource="http://www.ontologydesignpatterns.org/ont/dul/DUL.owl#SocialAgent"/>
        <rdfs:range rdf:resource="http://www.semanticweb.org/mguen/ontologies/2024/0/CognitiveBiasOntology/ostrich_effect#CopingStrategy"/>
        <rdfs:comment>This property indicates the coping strategies used by the individual to deal with the negative information.</rdfs:comment>
    </owl:ObjectProperty>
    


    <!-- http://etna.istc.cnr.it/framester2/data/framestercore/Avoiding -->

    <owl:ObjectProperty rdf:about="http://etna.istc.cnr.it/framester2/data/framestercore/Avoiding">
        <rdfs:domain rdf:resource="http://www.ontologydesignpatterns.org/ont/dul/DUL.owl#SocialAgent"/>
        <rdfs:range>
            <owl:Class>
                <owl:intersectionOf rdf:parseType="Collection">
                    <rdf:Description rdf:about="http://etna.istc.cnr.it/framester2/data/framestercore/Information"/>
                    <owl:Restriction>
                        <owl:onProperty rdf:resource="http://www.semanticweb.org/mguen/ontologies/2024/0/CognitiveBiasOntology/ostrich_effect#isNegative"/>
                        <owl:hasValue rdf:datatype="http://www.w3.org/2001/XMLSchema#boolean">true</owl:hasValue>
                    </owl:Restriction>
                </owl:intersectionOf>
            </owl:Class>
        </rdfs:range>
        <rdfs:comment>This property indicates that the individual is avoiding the negative information.</rdfs:comment>
    </owl:ObjectProperty>
    


    <!-- http://etna.istc.cnr.it/framester2/data/framestercore/Feeling -->

    <owl:ObjectProperty rdf:about="http://etna.istc.cnr.it/framester2/data/framestercore/Feeling">
        <rdfs:domain rdf:resource="http://www.ontologydesignpatterns.org/ont/dul/DUL.owl#SocialAgent"/>
        <rdfs:range rdf:resource="http://etna.istc.cnr.it/framester2/data/framestercore/Feeling"/>
    </owl:ObjectProperty>
    


    <!-- http://krisnadhi.github.io/onto/event.owl#hasInformationObject -->

    <owl:ObjectProperty rdf:about="http://krisnadhi.github.io/onto/event.owl#hasInformationObject">
        <rdfs:domain rdf:resource="http://www.ontologydesignpatterns.org/ont/dul/DUL.owl#SocialAgent"/>
        <rdfs:range rdf:resource="http://krisnadhi.github.io/onto/event.owl#InformationObject"/>
        <rdfs:comment>Property relating Event to InformationObject in this pattern. The domain of this property is not restricted to Event since it is possible that non-event to have an information object. The range is always InformationObject since it makes no sense to have a property named hasInformationObject to point to anything other than information object</rdfs:comment>
    </owl:ObjectProperty>
    


    <!-- http://www.ontology.se/odp/content/owl/Action.owl#has_consequence -->

    <owl:ObjectProperty rdf:about="http://www.ontology.se/odp/content/owl/Action.owl#has_consequence">
        <rdfs:domain>
            <owl:Class>
                <owl:unionOf rdf:parseType="Collection">
                    <rdf:Description rdf:about="http://etna.istc.cnr.it/framester2/data/framestercore/Feeling"/>
                    <rdf:Description rdf:about="http://etna.istc.cnr.it/framester2/data/framestercore/Information"/>
                    <owl:Class>
                        <owl:intersectionOf rdf:parseType="Collection">
                            <rdf:Description rdf:about="http://descartes-core.org/ontologies/activities/1.0/ActivityPattern.owl#Outcome"/>
                            <owl:Restriction>
                                <owl:onProperty rdf:resource="http://www.semanticweb.org/mguen/ontologies/2024/0/CognitiveBiasOntology/ostrich_effect#isPositive"/>
                                <owl:hasValue rdf:datatype="http://www.w3.org/2001/XMLSchema#boolean">true</owl:hasValue>
                            </owl:Restriction>
                        </owl:intersectionOf>
                    </owl:Class>
                </owl:unionOf>
            </owl:Class>
        </rdfs:domain>
        <rdfs:range>
            <owl:Class>
                <owl:unionOf rdf:parseType="Collection">
                    <rdf:Description rdf:about="http://etna.istc.cnr.it/framester2/data/framestercore/Feeling"/>
                    <rdf:Description rdf:about="http://www.semanticweb.org/mguen/ontologies/2024/0/CognitiveBiasOntology/ostrich_effect#Behavior"/>
                    <rdf:Description rdf:about="http://www.semanticweb.org/mguen/ontologies/2024/0/CognitiveBiasOntology/ostrich_effect#CopingStrategy"/>
                </owl:unionOf>
            </owl:Class>
        </rdfs:range>
        <rdfs:comment>(owl:TransitiveProperty) A causal relation between actions, i.e. one action is the cause of another action. For example, the action of &quot;swimming&quot; is a consequence of &quot;jumping into deep water&quot;. The property is transitive.</rdfs:comment>
        <rdfs:comment>The statement in the domain section want to express that only an Outcome that is positive can lead to a coping strategy.</rdfs:comment>
    </owl:ObjectProperty>
    


    <!-- http://www.ontologydesignpatterns.org/cp/owl/situation.owl#hasSetting -->

    <owl:ObjectProperty rdf:about="http://www.ontologydesignpatterns.org/cp/owl/situation.owl#hasSetting">
        <rdfs:domain rdf:resource="http://etna.istc.cnr.it/framester2/data/framestercore/Information"/>
        <rdfs:range rdf:resource="http://www.ontologydesignpatterns.org/cp/owl/situation.owl#Situation"/>
        <rdfs:comment>This property links the negative information to the context in which it exists.</rdfs:comment>
    </owl:ObjectProperty>
    


    <!-- 
    ///////////////////////////////////////////////////////////////////////////////////////
    //
    // Data properties
    //
    ///////////////////////////////////////////////////////////////////////////////////////
     -->

    


    <!-- http://www.semanticweb.org/mguen/ontologies/2024/0/CognitiveBiasOntology/ostrich_effect#isConfrontational -->

    <owl:DatatypeProperty rdf:about="http://www.semanticweb.org/mguen/ontologies/2024/0/CognitiveBiasOntology/ostrich_effect#isConfrontational">
        <rdfs:domain rdf:resource="http://www.semanticweb.org/mguen/ontologies/2024/0/CognitiveBiasOntology/ostrich_effect#Behavior"/>
        <rdfs:range rdf:resource="http://www.w3.org/2001/XMLSchema#boolean"/>
        <rdfs:comment>Denotes if the Behavior conducted by the SocialAgent is confrontational or not, leading to respectively a positive or negative outcome.</rdfs:comment>
    </owl:DatatypeProperty>
    


    <!-- http://www.semanticweb.org/mguen/ontologies/2024/0/CognitiveBiasOntology/ostrich_effect#isNegative -->

    <owl:DatatypeProperty rdf:about="http://www.semanticweb.org/mguen/ontologies/2024/0/CognitiveBiasOntology/ostrich_effect#isNegative">
        <rdfs:domain rdf:resource="http://etna.istc.cnr.it/framester2/data/framestercore/Information"/>
        <rdfs:range rdf:resource="http://www.w3.org/2001/XMLSchema#boolean"/>
        <rdfs:comment>This data property aim to express if the information that are related to the SocialAgent&apos;s interest are negative or not.</rdfs:comment>
    </owl:DatatypeProperty>
    


    <!-- http://www.semanticweb.org/mguen/ontologies/2024/0/CognitiveBiasOntology/ostrich_effect#isPositive -->

    <owl:DatatypeProperty rdf:about="http://www.semanticweb.org/mguen/ontologies/2024/0/CognitiveBiasOntology/ostrich_effect#isPositive">
        <rdfs:domain>
            <owl:Class>
                <owl:unionOf rdf:parseType="Collection">
                    <rdf:Description rdf:about="http://descartes-core.org/ontologies/activities/1.0/ActivityPattern.owl#Outcome"/>
                    <rdf:Description rdf:about="http://etna.istc.cnr.it/framester2/data/framestercore/Feeling"/>
                </owl:unionOf>
            </owl:Class>
        </rdfs:domain>
        <rdfs:range rdf:resource="http://www.w3.org/2001/XMLSchema#boolean"/>
        <rdfs:comment>Denotes if the Feeling the SocialAgent is feeling or the Outcome is positive or not</rdfs:comment>
    </owl:DatatypeProperty>
    


    <!-- http://www.semanticweb.org/mguen/ontologies/2024/0/CognitiveBiasOntology/ostrich_effect#isStressful -->

    <owl:DatatypeProperty rdf:about="http://www.semanticweb.org/mguen/ontologies/2024/0/CognitiveBiasOntology/ostrich_effect#isStressful">
        <rdfs:domain rdf:resource="http://www.ontologydesignpatterns.org/cp/owl/situation.owl#Situation"/>
        <rdfs:range rdf:resource="http://www.w3.org/2001/XMLSchema#boolean"/>
        <rdfs:comment>this property denote if the situation is stressful or not</rdfs:comment>
    </owl:DatatypeProperty>
    


    <!-- 
    ///////////////////////////////////////////////////////////////////////////////////////
    //
    // Classes
    //
    ///////////////////////////////////////////////////////////////////////////////////////
     -->

    


    <!-- http://descartes-core.org/ontologies/activities/1.0/ActivityPattern.owl#Outcome -->

    <owl:Class rdf:about="http://descartes-core.org/ontologies/activities/1.0/ActivityPattern.owl#Outcome">
        <rdfs:comment>Represents the result or consequence of an individualâ€™s behavior. In the context of the Ostrich Effect, the outcome could be the eventual confrontation of the negative information and the emotional response that follows.</rdfs:comment>
    </owl:Class>
    


    <!-- http://etna.istc.cnr.it/framester2/data/framestercore/Feeling -->

    <owl:Class rdf:about="http://etna.istc.cnr.it/framester2/data/framestercore/Feeling"/>
    


    <!-- http://etna.istc.cnr.it/framester2/data/framestercore/Information -->

    <owl:Class rdf:about="http://etna.istc.cnr.it/framester2/data/framestercore/Information">
        <rdfs:subClassOf rdf:resource="http://krisnadhi.github.io/onto/event.owl#InformationObject"/>
        <rdfs:comment>The potentially distressing information that the individual is avoiding.</rdfs:comment>
    </owl:Class>
    


    <!-- http://krisnadhi.github.io/onto/event.owl#InformationObject -->

    <owl:Class rdf:about="http://krisnadhi.github.io/onto/event.owl#InformationObject">
        <rdfs:comment>An entity that encapsulates all descriptive or non-defining information of the corresponding event, e.g., names, additional identifiers, textual descriptions, etc. Should normally be aligned to a separate Information Object pattern.</rdfs:comment>
    </owl:Class>
    


    <!-- http://www.ontologydesignpatterns.org/cp/owl/situation.owl#Situation -->

    <owl:Class rdf:about="http://www.ontologydesignpatterns.org/cp/owl/situation.owl#Situation">
        <rdfs:comment>(owl:Class) A view on a set of entities. It can be seen as a &apos;relational context&apos;, reifying a relation.</rdfs:comment>
        <rdfs:comment>Thi class represent the context in which the negative informations are presented or relates to</rdfs:comment>
    </owl:Class>
    


    <!-- http://www.ontologydesignpatterns.org/ont/dul/DUL.owl#SocialAgent -->

    <owl:Class rdf:about="http://www.ontologydesignpatterns.org/ont/dul/DUL.owl#SocialAgent">
        <rdfs:comment>Any individual whose existence is granted simply by its social communicability and capability of action (through some PhysicalAgent).</rdfs:comment>
        <rdfs:comment>a SocialAgent is equivalent to an individual that has a hasFear value of false and experiences an Outcome that is a consequence of a ConfrontationBehavior.</rdfs:comment>
        <rdfs:comment>a SocialAgent is equivalent to an individual that has a hasFear value of true and is Avoiding some NegativeInformation.</rdfs:comment>
        <rdfs:comment>a SocialAgent is equivalent to an individual that has a hasFear value of true, is Avoiding some NegativeInformation, and experiences an Outcome that is a consequence of an AvoidanceBehavior</rdfs:comment>
    </owl:Class>
    


    <!-- http://www.semanticweb.org/mguen/ontologies/2024/0/CognitiveBiasOntology/ostrich_effect#Behavior -->

    <owl:Class rdf:about="http://www.semanticweb.org/mguen/ontologies/2024/0/CognitiveBiasOntology/ostrich_effect#Behavior">
        <rdfs:comment>Represents the behavior of confronting or avoiding negative information</rdfs:comment>
    </owl:Class>
    


    <!-- http://www.semanticweb.org/mguen/ontologies/2024/0/CognitiveBiasOntology/ostrich_effect#CopingStrategy -->

    <owl:Class rdf:about="http://www.semanticweb.org/mguen/ontologies/2024/0/CognitiveBiasOntology/ostrich_effect#CopingStrategy">
        <rdfs:comment>Represents the methods an individual uses to deal with stressful situations. In the context of the Ostrich Effect, the coping strategy could be the decision to confront the negative information and make a plan to improve the situation.</rdfs:comment>
    </owl:Class>
    


    <!-- 
    ///////////////////////////////////////////////////////////////////////////////////////
    //
    // Individuals
    //
    ///////////////////////////////////////////////////////////////////////////////////////
     -->

    


    <!-- http://www.semanticweb.org/mguen/ontologies/2024/0/CognitiveBiasOntology/ostrich_effect#AcademicSetting -->

    <owl:NamedIndividual rdf:about="http://www.semanticweb.org/mguen/ontologies/2024/0/CognitiveBiasOntology/ostrich_effect#AcademicSetting">
        <rdf:type rdf:resource="http://www.ontologydesignpatterns.org/cp/owl/situation.owl#Situation"/>
        <isStressful rdf:datatype="http://www.w3.org/2001/XMLSchema#boolean">true</isStressful>
    </owl:NamedIndividual>
    


    <!-- http://www.semanticweb.org/mguen/ontologies/2024/0/CognitiveBiasOntology/ostrich_effect#Alex -->

    <owl:NamedIndividual rdf:about="http://www.semanticweb.org/mguen/ontologies/2024/0/CognitiveBiasOntology/ostrich_effect#Alex">
        <rdf:type rdf:resource="http://www.ontologydesignpatterns.org/ont/dul/DUL.owl#SocialAgent"/>
        <en:uses rdf:resource="http://www.semanticweb.org/mguen/ontologies/2024/0/CognitiveBiasOntology/ostrich_effect#Alex&apos;sPlan"/>
        <fs:Avoiding rdf:resource="http://www.semanticweb.org/mguen/ontologies/2024/0/CognitiveBiasOntology/ostrich_effect#DataStructureGrade"/>
        <fs:Feeling rdf:resource="http://www.semanticweb.org/mguen/ontologies/2024/0/CognitiveBiasOntology/ostrich_effect#Alex&apos;sFear"/>
        <event:hasInformationObject rdf:resource="http://www.semanticweb.org/mguen/ontologies/2024/0/CognitiveBiasOntology/ostrich_effect#Grades"/>
    </owl:NamedIndividual>
    


    <!-- http://www.semanticweb.org/mguen/ontologies/2024/0/CognitiveBiasOntology/ostrich_effect#DataStructureGrade -->

    <owl:NamedIndividual rdf:about="http://www.semanticweb.org/mguen/ontologies/2024/0/CognitiveBiasOntology/ostrich_effect#DataStructureGrade">
        <rdf:type rdf:resource="http://etna.istc.cnr.it/framester2/data/framestercore/Information"/>
        <situation:hasSetting rdf:resource="http://www.semanticweb.org/mguen/ontologies/2024/0/CognitiveBiasOntology/ostrich_effect#AcademicSetting"/>
        <isNegative rdf:datatype="http://www.w3.org/2001/XMLSchema#boolean">true</isNegative>
    </owl:NamedIndividual>
    


    <!-- http://www.semanticweb.org/mguen/ontologies/2024/0/CognitiveBiasOntology/ostrich_effect#FinallyCheckingGrades -->

    <owl:NamedIndividual rdf:about="http://www.semanticweb.org/mguen/ontologies/2024/0/CognitiveBiasOntology/ostrich_effect#FinallyCheckingGrades">
        <rdf:type rdf:resource="http://www.semanticweb.org/mguen/ontologies/2024/0/CognitiveBiasOntology/ostrich_effect#Behavior"/>
        <ActivityPattern:produces rdf:resource="http://www.semanticweb.org/mguen/ontologies/2024/0/CognitiveBiasOntology/ostrich_effect#Realization"/>
        <isConfrontational rdf:datatype="http://www.w3.org/2001/XMLSchema#boolean">true</isConfrontational>
    </owl:NamedIndividual>
    


    <!-- http://www.semanticweb.org/mguen/ontologies/2024/0/CognitiveBiasOntology/ostrich_effect#Grades -->

    <owl:NamedIndividual rdf:about="http://www.semanticweb.org/mguen/ontologies/2024/0/CognitiveBiasOntology/ostrich_effect#Grades">
        <rdf:type rdf:resource="http://krisnadhi.github.io/onto/event.owl#InformationObject"/>
    </owl:NamedIndividual>
    


    <!-- http://www.semanticweb.org/mguen/ontologies/2024/0/CognitiveBiasOntology/ostrich_effect#MoreStressAndAnxiety -->

    <owl:NamedIndividual rdf:about="http://www.semanticweb.org/mguen/ontologies/2024/0/CognitiveBiasOntology/ostrich_effect#MoreStressAndAnxiety">
        <rdf:type rdf:resource="http://descartes-core.org/ontologies/activities/1.0/ActivityPattern.owl#Outcome"/>
        <isPositive rdf:datatype="http://www.w3.org/2001/XMLSchema#boolean">false</isPositive>
    </owl:NamedIndividual>
    


    <!-- http://www.semanticweb.org/mguen/ontologies/2024/0/CognitiveBiasOntology/ostrich_effect#NotCheckingGrades -->

    <owl:NamedIndividual rdf:about="http://www.semanticweb.org/mguen/ontologies/2024/0/CognitiveBiasOntology/ostrich_effect#NotCheckingGrades">
        <rdf:type rdf:resource="http://www.semanticweb.org/mguen/ontologies/2024/0/CognitiveBiasOntology/ostrich_effect#Behavior"/>
        <ActivityPattern:produces rdf:resource="http://www.semanticweb.org/mguen/ontologies/2024/0/CognitiveBiasOntology/ostrich_effect#MoreStressAndAnxiety"/>
        <isConfrontational rdf:datatype="http://www.w3.org/2001/XMLSchema#boolean">false</isConfrontational>
    </owl:NamedIndividual>
    


    <!-- http://www.semanticweb.org/mguen/ontologies/2024/0/CognitiveBiasOntology/ostrich_effect#Realization -->

    <owl:NamedIndividual rdf:about="http://www.semanticweb.org/mguen/ontologies/2024/0/CognitiveBiasOntology/ostrich_effect#Realization">
        <rdf:type rdf:resource="http://descartes-core.org/ontologies/activities/1.0/ActivityPattern.owl#Outcome"/>
        <Action:has_consequence rdf:resource="http://www.semanticweb.org/mguen/ontologies/2024/0/CognitiveBiasOntology/ostrich_effect#Alex&apos;sPlan"/>
        <isPositive rdf:datatype="http://www.w3.org/2001/XMLSchema#boolean">true</isPositive>
    </owl:NamedIndividual>
    


    <!-- http://www.semanticweb.org/mguen/ontologies/2024/0/CognitiveBiasOntology/ostrich_effect#Alex&apos;sBravery -->

    <owl:NamedIndividual rdf:about="http://www.semanticweb.org/mguen/ontologies/2024/0/CognitiveBiasOntology/ostrich_effect#Alex&apos;sBravery">
        <rdf:type rdf:resource="http://etna.istc.cnr.it/framester2/data/framestercore/Feeling"/>
        <Action:has_consequence rdf:resource="http://www.semanticweb.org/mguen/ontologies/2024/0/CognitiveBiasOntology/ostrich_effect#FinallyCheckingGrades"/>
        <isPositive rdf:datatype="http://www.w3.org/2001/XMLSchema#boolean">true</isPositive>
    </owl:NamedIndividual>
    


    <!-- http://www.semanticweb.org/mguen/ontologies/2024/0/CognitiveBiasOntology/ostrich_effect#Alex&apos;sFear -->

    <owl:NamedIndividual rdf:about="http://www.semanticweb.org/mguen/ontologies/2024/0/CognitiveBiasOntology/ostrich_effect#Alex&apos;sFear">
        <rdf:type rdf:resource="http://etna.istc.cnr.it/framester2/data/framestercore/Feeling"/>
        <Action:has_consequence rdf:resource="http://www.semanticweb.org/mguen/ontologies/2024/0/CognitiveBiasOntology/ostrich_effect#NotCheckingGrades"/>
        <isPositive rdf:datatype="http://www.w3.org/2001/XMLSchema#boolean">false</isPositive>
    </owl:NamedIndividual>
    


    <!-- http://www.semanticweb.org/mguen/ontologies/2024/0/CognitiveBiasOntology/ostrich_effect#Alex&apos;sPlan -->

    <owl:NamedIndividual rdf:about="http://www.semanticweb.org/mguen/ontologies/2024/0/CognitiveBiasOntology/ostrich_effect#Alex&apos;sPlan">
        <rdf:type rdf:resource="http://www.semanticweb.org/mguen/ontologies/2024/0/CognitiveBiasOntology/ostrich_effect#CopingStrategy"/>
    </owl:NamedIndividual>
    


    <!-- 
    ///////////////////////////////////////////////////////////////////////////////////////
    //
    // Annotations
    //
    ///////////////////////////////////////////////////////////////////////////////////////
     -->

    <rdf:Description rdf:about="http://etna.istc.cnr.it/framester2/data/framestercore/Feeling">
        <rdfs:comment>In this frame an Experiencer experiences an Emotion or is in an Emotional_state. There can also be an Evaluation of the internal experiential state. John feels anger towards his mother. Martha feels angry. Dr. Hibbert feels good. Inalienably possessed aspects of the Experiencer frequently stand in for the Experiencer. Her heart felt angry.</rdfs:comment>
    </rdf:Description>
</rdf:RDF>



<!-- Generated by the OWL API (version 4.5.25.2023-02-15T19:15:49Z) https://github.com/owlcs/owlapi -->

