<?xml version="1.0"?>
<rdf:RDF xmlns="http://www.semanticweb.org/mguen/ontologies/2024/0/CognitiveBiasOntology/semmelweis_reflex#"
     xml:base="http://www.semanticweb.org/mguen/ontologies/2024/0/CognitiveBiasOntology/semmelweis_reflex"
     xmlns:ac="http://www.ontology.se/odp/content/owl/Action.owl"
     xmlns:st="http://www.ontologydesignpatterns.org/cp/owl/situation.owl"
     xmlns:acf="http://www.ontologydesignpatterns.org/ont/dul/DUL.owl"
     xmlns:acp="http://descartes-core.org/ontologies/activities/1.0/ActivityPattern.owl"
     xmlns:cbo="http://www.semanticweb.org/mguen/ontologies/2024/0/cognitive_bias_ontology_semmelweis_reflex/"
     xmlns:owl="http://www.w3.org/2002/07/owl#"
     xmlns:rdf="http://www.w3.org/1999/02/22-rdf-syntax-ns#"
     xmlns:xml="http://www.w3.org/XML/1998/namespace"
     xmlns:xsd="http://www.w3.org/2001/XMLSchema#"
     xmlns:rdfs="http://www.w3.org/2000/01/rdf-schema#"
     xmlns:terms="http://purl.org/dc/terms/"
     xmlns:Action="http://www.ontology.se/odp/content/owl/Action.owl#"
     xmlns:situation="http://www.ontologydesignpatterns.org/cp/owl/situation.owl#"
     xmlns:dbpedia-owl="https://en.wiktionary.org/wiki/"
     xmlns:semmelweis_reflex="http://www.semanticweb.org/mguen/ontologies/2024/0/CognitiveBiasOntology/semmelweis_reflex#">
    <owl:Ontology rdf:about="http://www.semanticweb.org/mguen/ontologies/2024/0/CognitiveBiasOntology/semmelweis_reflex">
        <terms:creator>12-02-2024</terms:creator>
        <terms:creator>Matteo Guenci</terms:creator>
        <terms:description>The Semmelweiss Reflex Ontology</terms:description>
        <hasComponent>http://descartes-core.org/ontologies/activities/1.0/ActivityPattern.owl</hasComponent>
        <hasComponent>http://www.ontology.se/odp/content/owl/Action.owl</hasComponent>
        <hasComponent>http://www.ontologydesignpatterns.org/cp/owl/situation.owl</hasComponent>
        <hasComponent>http://www.ontologydesignpatterns.org/ont/dul/DUL.owl</hasComponent>
        <user_story>Meet John, a middle-aged man who has been feeling persistently sad and uninterested in his usual activities for several weeks. His friends notice these changes and suggest that he might be dealing with depression, a common mental health condition. They recommend that he seek help from a mental health professional.

However, John has always held the belief that mental health issues are a sign of weakness and that they can be overcome simply by &quot;toughening up&quot;. He rejects the idea that he could be suffering from depression and refuses to consider therapy, despite numerous studies showing its effectiveness in treating mental health conditions.

Over time, John&apos;s symptoms worsen, and his quality of life deteriorates. He struggles at work and in his personal relationships, and his physical health begins to decline. Despite the clear evidence that he needs help, John&apos;s Semmelweis Reflex prevents him from accepting the psychological research and seeking the treatment he needs. Eventually John, through a lot of help and noticing his deteriorating quality of life, seeks help and this choice lead to a better quality of life. This story illustrates how the Semmelweis Reflex can lead to harmful outcomes when individuals reject established scientific findings due to pre-existing beliefs or biases.</user_story>
        <rdfs:comment>The Semmelweis Reflex, also known as the Semmelweis Effect, is a metaphor for the reflex-like tendency to reject new evidence or new knowledge because it contradicts established norms, beliefs, or paradigms. This term is named after Ignaz Semmelweis, a Hungarian physician who discovered in 1847 that childbed fever mortality rates fell significantly when doctors disinfected their hands with a chlorine solution before moving from one patient to another¹. Despite the empirical evidence, his fellow doctors rejected his hand-washing suggestions, often for non-medical reasons. This phenomenon can impede scientific advancement and progress by rejecting new ideas and discoveries².</rdfs:comment>
    </owl:Ontology>
    


    <!-- 
    ///////////////////////////////////////////////////////////////////////////////////////
    //
    // Annotation properties
    //
    ///////////////////////////////////////////////////////////////////////////////////////
     -->

    


    <!-- http://purl.org/dc/terms/created -->

    <owl:AnnotationProperty rdf:about="http://purl.org/dc/terms/created"/>
    


    <!-- http://purl.org/dc/terms/creator -->

    <owl:AnnotationProperty rdf:about="http://purl.org/dc/terms/creator"/>
    


    <!-- http://purl.org/dc/terms/description -->

    <owl:AnnotationProperty rdf:about="http://purl.org/dc/terms/description"/>
    


    <!-- http://www.semanticweb.org/mguen/ontologies/2024/0/CognitiveBiasOntology/semmelweis_reflex#hasComponent -->

    <owl:AnnotationProperty rdf:about="http://www.semanticweb.org/mguen/ontologies/2024/0/CognitiveBiasOntology/semmelweis_reflex#hasComponent"/>
    


    <!-- http://www.semanticweb.org/mguen/ontologies/2024/0/CognitiveBiasOntology/semmelweis_reflex#user_story -->

    <owl:AnnotationProperty rdf:about="http://www.semanticweb.org/mguen/ontologies/2024/0/CognitiveBiasOntology/semmelweis_reflex#user_story"/>
    


    <!-- 
    ///////////////////////////////////////////////////////////////////////////////////////
    //
    // Object Properties
    //
    ///////////////////////////////////////////////////////////////////////////////////////
     -->

    


    <!-- http://www.ontology.se/odp/content/owl/Action.owl#has_consequence -->

    <owl:ObjectProperty rdf:about="http://www.ontology.se/odp/content/owl/Action.owl#has_consequence">
        <rdfs:domain rdf:resource="http://www.ontology.se/odp/content/owl/Action.owl#Action"/>
        <rdfs:range rdf:resource="http://descartes-core.org/ontologies/activities/1.0/ActivityPattern.owl#Outcome"/>
        <rdfs:comment>(owl:TransitiveProperty) A causal relation between actions, i.e. one action is the cause of another action. For example, the action of &quot;swimming&quot; is a consequence of &quot;jumping into deep water&quot;. The property is transitive.</rdfs:comment>
    </owl:ObjectProperty>
    


    <!-- http://www.ontologydesignpatterns.org/cp/owl/situation.owl#hasSetting -->

    <owl:ObjectProperty rdf:about="http://www.ontologydesignpatterns.org/cp/owl/situation.owl#hasSetting">
        <rdfs:domain rdf:resource="http://www.ontologydesignpatterns.org/ont/dul/DUL.owl#SocialAgent"/>
        <rdfs:range rdf:resource="http://www.semanticweb.org/mguen/ontologies/2024/0/CognitiveBiasOntology/semmelweis_reflex#Environment"/>
        <rdfs:comment>(owl:ObjectProperty) A relation between entities and situations, e.g. &apos;this morning I&apos;ve prepared my coffee with a new fantastic Arabica&apos; (i.e.: (an amount of) a new fantastic Arabica hasSetting the preparation of my coffee this morning).</rdfs:comment>
        <rdfs:comment>Represent theconnection of the Social agent to the condition it is in</rdfs:comment>
    </owl:ObjectProperty>
    


    <!-- http://www.semanticweb.org/mguen/ontologies/2024/0/CognitiveBiasOntology/semmelweis_reflex#contradicts -->

    <owl:ObjectProperty rdf:about="http://www.semanticweb.org/mguen/ontologies/2024/0/CognitiveBiasOntology/semmelweis_reflex#contradicts">
        <rdfs:domain rdf:resource="http://www.semanticweb.org/mguen/ontologies/2024/0/CognitiveBiasOntology/semmelweis_reflex#Perception"/>
        <rdfs:range rdf:resource="http://www.semanticweb.org/mguen/ontologies/2024/0/CognitiveBiasOntology/semmelweis_reflex#Fact"/>
        <owl:propertyDisjointWith rdf:resource="http://www.semanticweb.org/mguen/ontologies/2024/0/CognitiveBiasOntology/semmelweis_reflex#supports"/>
        <rdfs:comment>Links a perception to the fact it contradicts.</rdfs:comment>
    </owl:ObjectProperty>
    


    <!-- http://www.semanticweb.org/mguen/ontologies/2024/0/CognitiveBiasOntology/semmelweis_reflex#holds -->

    <owl:ObjectProperty rdf:about="http://www.semanticweb.org/mguen/ontologies/2024/0/CognitiveBiasOntology/semmelweis_reflex#holds">
        <rdfs:domain rdf:resource="http://www.ontologydesignpatterns.org/ont/dul/DUL.owl#SocialAgent"/>
        <rdfs:range rdf:resource="http://www.semanticweb.org/mguen/ontologies/2024/0/CognitiveBiasOntology/semmelweis_reflex#Perception"/>
        <rdfs:comment>Links an entity to the perception it holds.</rdfs:comment>
    </owl:ObjectProperty>
    


    <!-- http://www.semanticweb.org/mguen/ontologies/2024/0/CognitiveBiasOntology/semmelweis_reflex#isAffectedBy -->

    <owl:ObjectProperty rdf:about="http://www.semanticweb.org/mguen/ontologies/2024/0/CognitiveBiasOntology/semmelweis_reflex#isAffectedBy">
        <rdfs:domain rdf:resource="http://www.ontologydesignpatterns.org/ont/dul/DUL.owl#SocialAgent"/>
        <rdfs:range rdf:resource="http://www.ontologydesignpatterns.org/cp/owl/situation.owl#Situation"/>
        <rdfs:comment>Links an entity to the environment it is affected by.</rdfs:comment>
    </owl:ObjectProperty>
    


    <!-- http://www.semanticweb.org/mguen/ontologies/2024/0/CognitiveBiasOntology/semmelweis_reflex#rejects -->

    <owl:ObjectProperty rdf:about="http://www.semanticweb.org/mguen/ontologies/2024/0/CognitiveBiasOntology/semmelweis_reflex#rejects">
        <rdfs:domain rdf:resource="http://www.ontologydesignpatterns.org/ont/dul/DUL.owl#SocialAgent"/>
        <rdfs:range rdf:resource="http://www.semanticweb.org/mguen/ontologies/2024/0/CognitiveBiasOntology/semmelweis_reflex#Fact"/>
        <rdfs:comment>links the SocialAgent to the fact he/she rejects because of the perception he/she has.</rdfs:comment>
    </owl:ObjectProperty>
    


    <!-- http://www.semanticweb.org/mguen/ontologies/2024/0/CognitiveBiasOntology/semmelweis_reflex#requires -->

    <owl:ObjectProperty rdf:about="http://www.semanticweb.org/mguen/ontologies/2024/0/CognitiveBiasOntology/semmelweis_reflex#requires">
        <rdfs:domain rdf:resource="http://www.ontologydesignpatterns.org/ont/dul/DUL.owl#SocialAgent"/>
        <rdfs:range rdf:resource="http://www.ontology.se/odp/content/owl/Action.owl#Action"/>
        <rdfs:comment>Links an entity to the action it needs to take.</rdfs:comment>
    </owl:ObjectProperty>
    


    <!-- http://www.semanticweb.org/mguen/ontologies/2024/0/CognitiveBiasOntology/semmelweis_reflex#supports -->

    <owl:ObjectProperty rdf:about="http://www.semanticweb.org/mguen/ontologies/2024/0/CognitiveBiasOntology/semmelweis_reflex#supports">
        <rdfs:domain>
            <owl:Class>
                <owl:unionOf rdf:parseType="Collection">
                    <rdf:Description rdf:about="http://www.semanticweb.org/mguen/ontologies/2024/0/CognitiveBiasOntology/semmelweis_reflex#Fact"/>
                    <rdf:Description rdf:about="http://www.semanticweb.org/mguen/ontologies/2024/0/CognitiveBiasOntology/semmelweis_reflex#Perception"/>
                </owl:unionOf>
            </owl:Class>
        </rdfs:domain>
        <rdfs:range rdf:resource="http://www.ontology.se/odp/content/owl/Action.owl#Action"/>
        <rdfs:comment>Links a fact to the action it supports.</rdfs:comment>
    </owl:ObjectProperty>
    


    <!-- 
    ///////////////////////////////////////////////////////////////////////////////////////
    //
    // Data properties
    //
    ///////////////////////////////////////////////////////////////////////////////////////
     -->

    


    <!-- http://www.semanticweb.org/mguen/ontologies/2024/0/CognitiveBiasOntology/semmelweis_reflex#isAware -->

    <owl:DatatypeProperty rdf:about="http://www.semanticweb.org/mguen/ontologies/2024/0/CognitiveBiasOntology/semmelweis_reflex#isAware">
        <rdfs:domain rdf:resource="http://www.ontologydesignpatterns.org/ont/dul/DUL.owl#SocialAgent"/>
        <rdfs:range rdf:resource="http://www.w3.org/2001/XMLSchema#boolean"/>
        <rdfs:comment>Indicates whether the entity is aware of their state.</rdfs:comment>
    </owl:DatatypeProperty>
    


    <!-- http://www.semanticweb.org/mguen/ontologies/2024/0/CognitiveBiasOntology/semmelweis_reflex#isChronic -->

    <owl:DatatypeProperty rdf:about="http://www.semanticweb.org/mguen/ontologies/2024/0/CognitiveBiasOntology/semmelweis_reflex#isChronic">
        <rdfs:domain rdf:resource="http://www.ontologydesignpatterns.org/cp/owl/situation.owl#Situation"/>
        <rdfs:range rdf:resource="http://www.w3.org/2001/XMLSchema#boolean"/>
        <rdfs:comment>Indicates whether the state is chronic or long-lasting.</rdfs:comment>
    </owl:DatatypeProperty>
    


    <!-- http://www.semanticweb.org/mguen/ontologies/2024/0/CognitiveBiasOntology/semmelweis_reflex#isComplex -->

    <owl:DatatypeProperty rdf:about="http://www.semanticweb.org/mguen/ontologies/2024/0/CognitiveBiasOntology/semmelweis_reflex#isComplex">
        <rdfs:domain>
            <owl:Class>
                <owl:unionOf rdf:parseType="Collection">
                    <rdf:Description rdf:about="http://www.ontology.se/odp/content/owl/Action.owl#Action"/>
                    <rdf:Description rdf:about="http://www.semanticweb.org/mguen/ontologies/2024/0/CognitiveBiasOntology/semmelweis_reflex#Environment"/>
                </owl:unionOf>
            </owl:Class>
        </rdfs:domain>
        <rdfs:range rdf:resource="http://www.w3.org/2001/XMLSchema#boolean"/>
        <rdfs:comment>Indicates whether the environment, or the action to perform, is complex or challenging.</rdfs:comment>
    </owl:DatatypeProperty>
    


    <!-- http://www.semanticweb.org/mguen/ontologies/2024/0/CognitiveBiasOntology/semmelweis_reflex#isNegative -->

    <owl:DatatypeProperty rdf:about="http://www.semanticweb.org/mguen/ontologies/2024/0/CognitiveBiasOntology/semmelweis_reflex#isNegative">
        <rdfs:domain rdf:resource="http://descartes-core.org/ontologies/activities/1.0/ActivityPattern.owl#Outcome"/>
        <rdfs:range rdf:resource="http://www.w3.org/2001/XMLSchema#boolean"/>
        <rdfs:comment>Indicates whether the consequence is negative or harmful.</rdfs:comment>
    </owl:DatatypeProperty>
    


    <!-- http://www.semanticweb.org/mguen/ontologies/2024/0/CognitiveBiasOntology/semmelweis_reflex#isStrong -->

    <owl:DatatypeProperty rdf:about="http://www.semanticweb.org/mguen/ontologies/2024/0/CognitiveBiasOntology/semmelweis_reflex#isStrong">
        <rdfs:domain rdf:resource="http://www.semanticweb.org/mguen/ontologies/2024/0/CognitiveBiasOntology/semmelweis_reflex#Perception"/>
        <rdfs:range rdf:resource="http://www.w3.org/2001/XMLSchema#boolean"/>
        <rdfs:comment>Indicates the strength or intensity of the perception.</rdfs:comment>
    </owl:DatatypeProperty>
    


    <!-- http://www.semanticweb.org/mguen/ontologies/2024/0/CognitiveBiasOntology/semmelweis_reflex#isVerified -->

    <owl:DatatypeProperty rdf:about="http://www.semanticweb.org/mguen/ontologies/2024/0/CognitiveBiasOntology/semmelweis_reflex#isVerified">
        <rdfs:domain rdf:resource="http://www.semanticweb.org/mguen/ontologies/2024/0/CognitiveBiasOntology/semmelweis_reflex#Fact"/>
        <rdfs:range rdf:resource="http://www.w3.org/2001/XMLSchema#boolean"/>
        <rdfs:comment>Indicates whether the fact is verified or confirmed.</rdfs:comment>
    </owl:DatatypeProperty>
    


    <!-- 
    ///////////////////////////////////////////////////////////////////////////////////////
    //
    // Classes
    //
    ///////////////////////////////////////////////////////////////////////////////////////
     -->

    


    <!-- http://descartes-core.org/ontologies/activities/1.0/ActivityPattern.owl#Outcome -->

    <owl:Class rdf:about="http://descartes-core.org/ontologies/activities/1.0/ActivityPattern.owl#Outcome">
        <rdfs:comment>Represents the result or effect of an action.</rdfs:comment>
        <rdfs:comment>an Outcome is negative if the action needed and the environment is complex and the SocialAgent is not aware of his/her situation.</rdfs:comment>
    </owl:Class>
    


    <!-- http://www.ontology.se/odp/content/owl/Action.owl#Action -->

    <owl:Class rdf:about="http://www.ontology.se/odp/content/owl/Action.owl#Action">
        <owl:equivalentClass>
            <owl:Class>
                <owl:intersectionOf rdf:parseType="Collection">
                    <rdf:Description rdf:about="http://www.ontology.se/odp/content/owl/Action.owl#Action"/>
                    <owl:Restriction>
                        <owl:onProperty rdf:resource="http://www.ontology.se/odp/content/owl/Action.owl#has_consequence"/>
                        <owl:someValuesFrom>
                            <owl:Class>
                                <owl:intersectionOf rdf:parseType="Collection">
                                    <rdf:Description rdf:about="http://descartes-core.org/ontologies/activities/1.0/ActivityPattern.owl#Outcome"/>
                                    <owl:Restriction>
                                        <owl:onProperty rdf:resource="http://www.semanticweb.org/mguen/ontologies/2024/0/CognitiveBiasOntology/semmelweis_reflex#isNegative"/>
                                        <owl:hasValue rdf:datatype="http://www.w3.org/2001/XMLSchema#boolean">false</owl:hasValue>
                                    </owl:Restriction>
                                </owl:intersectionOf>
                            </owl:Class>
                        </owl:someValuesFrom>
                    </owl:Restriction>
                    <owl:Restriction>
                        <owl:onProperty rdf:resource="http://www.semanticweb.org/mguen/ontologies/2024/0/CognitiveBiasOntology/semmelweis_reflex#isComplex"/>
                        <owl:hasValue rdf:datatype="http://www.w3.org/2001/XMLSchema#boolean">true</owl:hasValue>
                    </owl:Restriction>
                </owl:intersectionOf>
            </owl:Class>
        </owl:equivalentClass>
        <owl:equivalentClass>
            <owl:Class>
                <owl:intersectionOf rdf:parseType="Collection">
                    <rdf:Description rdf:about="http://www.ontology.se/odp/content/owl/Action.owl#Action"/>
                    <owl:Restriction>
                        <owl:onProperty rdf:resource="http://www.ontology.se/odp/content/owl/Action.owl#has_consequence"/>
                        <owl:someValuesFrom>
                            <owl:Class>
                                <owl:intersectionOf rdf:parseType="Collection">
                                    <rdf:Description rdf:about="http://descartes-core.org/ontologies/activities/1.0/ActivityPattern.owl#Outcome"/>
                                    <owl:Restriction>
                                        <owl:onProperty rdf:resource="http://www.semanticweb.org/mguen/ontologies/2024/0/CognitiveBiasOntology/semmelweis_reflex#isNegative"/>
                                        <owl:hasValue rdf:datatype="http://www.w3.org/2001/XMLSchema#boolean">true</owl:hasValue>
                                    </owl:Restriction>
                                </owl:intersectionOf>
                            </owl:Class>
                        </owl:someValuesFrom>
                    </owl:Restriction>
                    <owl:Restriction>
                        <owl:onProperty rdf:resource="http://www.semanticweb.org/mguen/ontologies/2024/0/CognitiveBiasOntology/semmelweis_reflex#isComplex"/>
                        <owl:hasValue rdf:datatype="http://www.w3.org/2001/XMLSchema#boolean">false</owl:hasValue>
                    </owl:Restriction>
                </owl:intersectionOf>
            </owl:Class>
        </owl:equivalentClass>
        <rdfs:comment>(owl:Class) The process of doing something. An action is performed by an agent. An action can be proposed (proposed actions make up a plan), implemented or abandoned, and it has a status and possibly one or more suspension periods. Actions can have consequences and can be dependent on other actions, e.g. the action of pouring water from a cup is dependent on the action to first fill the cup with water.</rdfs:comment>
        <rdfs:comment>The condition want to express that if the action is complex (e.g. going to theraphy) it will produce a positive outcome, the opposite conditon states that if the action is not complex (e.g. not going to theraphy) the outcome will be negative.

(this description doesn&apos;t want to simplify or minimize mental health problems that affect people by labeling actions as complex or not, but for the sake of this section of the cognitive bias ontology this choice has been made to express a linear flow of the logical steps this bias can lead to)</rdfs:comment>
    </owl:Class>
    


    <!-- http://www.ontologydesignpatterns.org/cp/owl/situation.owl#Situation -->

    <owl:Class rdf:about="http://www.ontologydesignpatterns.org/cp/owl/situation.owl#Situation">
        <rdfs:comment>(owl:Class) A view on a set of entities. It can be seen as a &apos;relational context&apos;, reifying a relation.</rdfs:comment>
        <rdfs:comment>Represents the surroundings or conditions in which an entity operates.</rdfs:comment>
    </owl:Class>
    


    <!-- http://www.ontologydesignpatterns.org/ont/dul/DUL.owl#SocialAgent -->

    <owl:Class rdf:about="http://www.ontologydesignpatterns.org/ont/dul/DUL.owl#SocialAgent">
        <owl:equivalentClass>
            <owl:Class>
                <owl:intersectionOf rdf:parseType="Collection">
                    <owl:Restriction>
                        <owl:onProperty rdf:resource="http://www.ontologydesignpatterns.org/cp/owl/situation.owl#hasSetting"/>
                        <owl:someValuesFrom>
                            <owl:Class>
                                <owl:intersectionOf rdf:parseType="Collection">
                                    <rdf:Description rdf:about="http://www.semanticweb.org/mguen/ontologies/2024/0/CognitiveBiasOntology/semmelweis_reflex#Environment"/>
                                    <owl:Restriction>
                                        <owl:onProperty rdf:resource="http://www.semanticweb.org/mguen/ontologies/2024/0/CognitiveBiasOntology/semmelweis_reflex#isComplex"/>
                                        <owl:hasValue rdf:datatype="http://www.w3.org/2001/XMLSchema#boolean">true</owl:hasValue>
                                    </owl:Restriction>
                                </owl:intersectionOf>
                            </owl:Class>
                        </owl:someValuesFrom>
                    </owl:Restriction>
                    <owl:Restriction>
                        <owl:onProperty rdf:resource="http://www.semanticweb.org/mguen/ontologies/2024/0/CognitiveBiasOntology/semmelweis_reflex#holds"/>
                        <owl:someValuesFrom>
                            <owl:Class>
                                <owl:intersectionOf rdf:parseType="Collection">
                                    <rdf:Description rdf:about="http://www.semanticweb.org/mguen/ontologies/2024/0/CognitiveBiasOntology/semmelweis_reflex#Perception"/>
                                    <owl:Restriction>
                                        <owl:onProperty rdf:resource="http://www.semanticweb.org/mguen/ontologies/2024/0/CognitiveBiasOntology/semmelweis_reflex#isStrong"/>
                                        <owl:hasValue rdf:datatype="http://www.w3.org/2001/XMLSchema#boolean">true</owl:hasValue>
                                    </owl:Restriction>
                                </owl:intersectionOf>
                            </owl:Class>
                        </owl:someValuesFrom>
                    </owl:Restriction>
                    <owl:Restriction>
                        <owl:onProperty rdf:resource="http://www.semanticweb.org/mguen/ontologies/2024/0/CognitiveBiasOntology/semmelweis_reflex#isAffectedBy"/>
                        <owl:someValuesFrom>
                            <owl:Class>
                                <owl:intersectionOf rdf:parseType="Collection">
                                    <rdf:Description rdf:about="http://www.ontologydesignpatterns.org/cp/owl/situation.owl#Situation"/>
                                    <owl:Restriction>
                                        <owl:onProperty rdf:resource="http://www.semanticweb.org/mguen/ontologies/2024/0/CognitiveBiasOntology/semmelweis_reflex#isChronic"/>
                                        <owl:hasValue rdf:datatype="http://www.w3.org/2001/XMLSchema#boolean">true</owl:hasValue>
                                    </owl:Restriction>
                                </owl:intersectionOf>
                            </owl:Class>
                        </owl:someValuesFrom>
                    </owl:Restriction>
                    <owl:Restriction>
                        <owl:onProperty rdf:resource="http://www.semanticweb.org/mguen/ontologies/2024/0/CognitiveBiasOntology/semmelweis_reflex#requires"/>
                        <owl:someValuesFrom>
                            <owl:Class>
                                <owl:intersectionOf rdf:parseType="Collection">
                                    <rdf:Description rdf:about="http://www.ontology.se/odp/content/owl/Action.owl#Action"/>
                                    <owl:Restriction>
                                        <owl:onProperty rdf:resource="http://www.semanticweb.org/mguen/ontologies/2024/0/CognitiveBiasOntology/semmelweis_reflex#isComplex"/>
                                        <owl:hasValue rdf:datatype="http://www.w3.org/2001/XMLSchema#boolean">true</owl:hasValue>
                                    </owl:Restriction>
                                </owl:intersectionOf>
                            </owl:Class>
                        </owl:someValuesFrom>
                    </owl:Restriction>
                    <owl:Restriction>
                        <owl:onProperty rdf:resource="http://www.semanticweb.org/mguen/ontologies/2024/0/CognitiveBiasOntology/semmelweis_reflex#isAware"/>
                        <owl:hasValue rdf:datatype="http://www.w3.org/2001/XMLSchema#boolean">false</owl:hasValue>
                    </owl:Restriction>
                </owl:intersectionOf>
            </owl:Class>
        </owl:equivalentClass>
        <rdfs:comment>(owl:Class) Any individual whose existence is granted simply by its social communicability and capability of action (through some PhysicalAgent)</rdfs:comment>
        <rdfs:comment>A SocialAgent is an individual who operates in a complex environment, faces chronic situations, and holds strong perceptions. They perform complex actions, which remain so even when facts are confirmed. Despite these challenges, they may not be fully aware of their circumstances. This paints a picture of resilience and adaptability in a complex world.

The rule provides a sufficient condition for being a SocialAgent, but it’s not a necessary condition. There could be SocialAgents that don’t meet these conditions</rdfs:comment>
    </owl:Class>
    


    <!-- http://www.semanticweb.org/mguen/ontologies/2024/0/CognitiveBiasOntology/semmelweis_reflex#Environment -->

    <owl:Class rdf:about="http://www.semanticweb.org/mguen/ontologies/2024/0/CognitiveBiasOntology/semmelweis_reflex#Environment">
        <rdfs:comment>Represents the surroundings or conditions in which an entity operates.</rdfs:comment>
    </owl:Class>
    


    <!-- http://www.semanticweb.org/mguen/ontologies/2024/0/CognitiveBiasOntology/semmelweis_reflex#Fact -->

    <owl:Class rdf:about="http://www.semanticweb.org/mguen/ontologies/2024/0/CognitiveBiasOntology/semmelweis_reflex#Fact">
        <rdfs:comment>Represents verified information or truth.</rdfs:comment>
    </owl:Class>
    


    <!-- http://www.semanticweb.org/mguen/ontologies/2024/0/CognitiveBiasOntology/semmelweis_reflex#Perception -->

    <owl:Class rdf:about="http://www.semanticweb.org/mguen/ontologies/2024/0/CognitiveBiasOntology/semmelweis_reflex#Perception">
        <rdfs:comment>Represents the way an entity thinks or understands something.</rdfs:comment>
    </owl:Class>
    


    <!-- 
    ///////////////////////////////////////////////////////////////////////////////////////
    //
    // Individuals
    //
    ///////////////////////////////////////////////////////////////////////////////////////
     -->

    


    <!-- http://www.semanticweb.org/mguen/ontologies/2024/0/CognitiveBiasOntology/semmelweis_reflex#BetterQualityOfLife -->

    <owl:NamedIndividual rdf:about="http://www.semanticweb.org/mguen/ontologies/2024/0/CognitiveBiasOntology/semmelweis_reflex#BetterQualityOfLife">
        <rdf:type rdf:resource="http://descartes-core.org/ontologies/activities/1.0/ActivityPattern.owl#Outcome"/>
        <isNegative rdf:datatype="http://www.w3.org/2001/XMLSchema#boolean">false</isNegative>
    </owl:NamedIndividual>
    


    <!-- http://www.semanticweb.org/mguen/ontologies/2024/0/CognitiveBiasOntology/semmelweis_reflex#DepressionIsCommon -->

    <owl:NamedIndividual rdf:about="http://www.semanticweb.org/mguen/ontologies/2024/0/CognitiveBiasOntology/semmelweis_reflex#DepressionIsCommon">
        <rdf:type rdf:resource="http://www.semanticweb.org/mguen/ontologies/2024/0/CognitiveBiasOntology/semmelweis_reflex#Fact"/>
        <supports rdf:resource="http://www.semanticweb.org/mguen/ontologies/2024/0/CognitiveBiasOntology/semmelweis_reflex#GoingToTheraphy"/>
        <isVerified rdf:datatype="http://www.w3.org/2001/XMLSchema#boolean">true</isVerified>
    </owl:NamedIndividual>
    


    <!-- http://www.semanticweb.org/mguen/ontologies/2024/0/CognitiveBiasOntology/semmelweis_reflex#DeterioratingQualityOfLife -->

    <owl:NamedIndividual rdf:about="http://www.semanticweb.org/mguen/ontologies/2024/0/CognitiveBiasOntology/semmelweis_reflex#DeterioratingQualityOfLife">
        <rdf:type rdf:resource="http://descartes-core.org/ontologies/activities/1.0/ActivityPattern.owl#Outcome"/>
        <isNegative rdf:datatype="http://www.w3.org/2001/XMLSchema#boolean">true</isNegative>
    </owl:NamedIndividual>
    


    <!-- http://www.semanticweb.org/mguen/ontologies/2024/0/CognitiveBiasOntology/semmelweis_reflex#GoingToTheraphy -->

    <owl:NamedIndividual rdf:about="http://www.semanticweb.org/mguen/ontologies/2024/0/CognitiveBiasOntology/semmelweis_reflex#GoingToTheraphy">
        <rdf:type rdf:resource="http://www.ontology.se/odp/content/owl/Action.owl#Action"/>
        <Action:has_consequence rdf:resource="http://www.semanticweb.org/mguen/ontologies/2024/0/CognitiveBiasOntology/semmelweis_reflex#BetterQualityOfLife"/>
        <isComplex rdf:datatype="http://www.w3.org/2001/XMLSchema#boolean">true</isComplex>
    </owl:NamedIndividual>
    


    <!-- http://www.semanticweb.org/mguen/ontologies/2024/0/CognitiveBiasOntology/semmelweis_reflex#John -->

    <owl:NamedIndividual rdf:about="http://www.semanticweb.org/mguen/ontologies/2024/0/CognitiveBiasOntology/semmelweis_reflex#John">
        <rdf:type rdf:resource="http://www.ontologydesignpatterns.org/ont/dul/DUL.owl#SocialAgent"/>
        <situation:hasSetting rdf:resource="http://www.semanticweb.org/mguen/ontologies/2024/0/CognitiveBiasOntology/semmelweis_reflex#John&apos;sWorkplace"/>
        <holds rdf:resource="http://www.semanticweb.org/mguen/ontologies/2024/0/CognitiveBiasOntology/semmelweis_reflex#MentalHealthIssuesAreWeakness"/>
        <isAffectedBy rdf:resource="http://www.semanticweb.org/mguen/ontologies/2024/0/CognitiveBiasOntology/semmelweis_reflex#PersistentSadness"/>
        <rejects rdf:resource="http://www.semanticweb.org/mguen/ontologies/2024/0/CognitiveBiasOntology/semmelweis_reflex#DepressionIsCommon"/>
        <requires rdf:resource="http://www.semanticweb.org/mguen/ontologies/2024/0/CognitiveBiasOntology/semmelweis_reflex#GoingToTheraphy"/>
    </owl:NamedIndividual>
    


    <!-- http://www.semanticweb.org/mguen/ontologies/2024/0/CognitiveBiasOntology/semmelweis_reflex#MentalHealthIssuesAreWeakness -->

    <owl:NamedIndividual rdf:about="http://www.semanticweb.org/mguen/ontologies/2024/0/CognitiveBiasOntology/semmelweis_reflex#MentalHealthIssuesAreWeakness">
        <rdf:type rdf:resource="http://www.semanticweb.org/mguen/ontologies/2024/0/CognitiveBiasOntology/semmelweis_reflex#Perception"/>
        <contradicts rdf:resource="http://www.semanticweb.org/mguen/ontologies/2024/0/CognitiveBiasOntology/semmelweis_reflex#DepressionIsCommon"/>
        <supports rdf:resource="http://www.semanticweb.org/mguen/ontologies/2024/0/CognitiveBiasOntology/semmelweis_reflex#RejectingTherapy"/>
        <isStrong rdf:datatype="http://www.w3.org/2001/XMLSchema#boolean">true</isStrong>
    </owl:NamedIndividual>
    


    <!-- http://www.semanticweb.org/mguen/ontologies/2024/0/CognitiveBiasOntology/semmelweis_reflex#PersistentSadness -->

    <owl:NamedIndividual rdf:about="http://www.semanticweb.org/mguen/ontologies/2024/0/CognitiveBiasOntology/semmelweis_reflex#PersistentSadness">
        <rdf:type rdf:resource="http://www.ontologydesignpatterns.org/cp/owl/situation.owl#Situation"/>
        <isChronic rdf:datatype="http://www.w3.org/2001/XMLSchema#boolean">true</isChronic>
    </owl:NamedIndividual>
    


    <!-- http://www.semanticweb.org/mguen/ontologies/2024/0/CognitiveBiasOntology/semmelweis_reflex#RejectingTherapy -->

    <owl:NamedIndividual rdf:about="http://www.semanticweb.org/mguen/ontologies/2024/0/CognitiveBiasOntology/semmelweis_reflex#RejectingTherapy">
        <rdf:type rdf:resource="http://www.ontology.se/odp/content/owl/Action.owl#Action"/>
        <Action:has_consequence rdf:resource="http://www.semanticweb.org/mguen/ontologies/2024/0/CognitiveBiasOntology/semmelweis_reflex#DeterioratingQualityOfLife"/>
        <isComplex rdf:datatype="http://www.w3.org/2001/XMLSchema#boolean">false</isComplex>
    </owl:NamedIndividual>
    


    <!-- http://www.semanticweb.org/mguen/ontologies/2024/0/CognitiveBiasOntology/semmelweis_reflex#John&apos;sWorkplace -->

    <owl:NamedIndividual rdf:about="http://www.semanticweb.org/mguen/ontologies/2024/0/CognitiveBiasOntology/semmelweis_reflex#John&apos;sWorkplace">
        <rdf:type rdf:resource="http://www.semanticweb.org/mguen/ontologies/2024/0/CognitiveBiasOntology/semmelweis_reflex#Environment"/>
        <isComplex rdf:datatype="http://www.w3.org/2001/XMLSchema#boolean">true</isComplex>
    </owl:NamedIndividual>
</rdf:RDF>



<!-- Generated by the OWL API (version 4.5.25.2023-02-15T19:15:49Z) https://github.com/owlcs/owlapi -->

