<?xml version="1.0"?>
<rdf:RDF xmlns="http://www.semanticweb.org/mguen/ontologies/2024/0/CognitiveBiasOntology/subjective_validation#"
     xml:base="http://www.semanticweb.org/mguen/ontologies/2024/0/CognitiveBiasOntology/subjective_validation"
     xmlns:ac="http://www.ontology.se/odp/content/owl/Action.owl"
     xmlns:ec="http://krisnadhi.github.io/onto/event.owl"
     xmlns:fs="http://etna.istc.cnr.it/framester2/data/framestercore/"
     xmlns:acf="http://www.ontologydesignpatterns.org/ont/dul/DUL.owl"
     xmlns:cbo="http://www.semanticweb.org/mguen/ontologies/2024/0/CognitiveBiasOntology/subjective_validation#"
     xmlns:owl="http://www.w3.org/2002/07/owl#"
     xmlns:rdf="http://www.w3.org/1999/02/22-rdf-syntax-ns#"
     xmlns:xml="http://www.w3.org/XML/1998/namespace"
     xmlns:xsd="http://www.w3.org/2001/XMLSchema#"
     xmlns:desc="http://www.ontologydesignpatterns.org/cp/owl/description.owl"
     xmlns:exob="https://raw.githubusercontent.com/eureadit/crowdsourcing-ontology/master/owl/crowdsourcing-evidences.owl.ttl"
     xmlns:rdfs="http://www.w3.org/2000/01/rdf-schema#"
     xmlns:wiki="https://en.wiktionary.org/"
     xmlns:terms="http://purl.org/dc/terms/"
     xmlns:dbpedia="https://www.dbpedia.org/">
    <owl:Ontology rdf:about="http://www.semanticweb.org/mguen/ontologies/2024/0/CognitiveBiasOntology/subjective_validation">
        <terms:created>10-02-2024</terms:created>
        <terms:creator>Matteo Guenci</terms:creator>
        <terms:description>Subjective Validation Ontology</terms:description>
        <terms:description>The Subjective Validation section of the Cognitive Bias Ontology.</terms:description>
        <hasComponent>http://ontologydesignpatterns.org/wiki/Submissions:Action</hasComponent>
        <hasComponent>http://ontologydesignpatterns.org/wiki/Submissions:EventCore</hasComponent>
        <hasComponent>http://www.ontologydesignpatterns.org/ont/dul/DUL.owl</hasComponent>
        <hasComponent>https://raw.githubusercontent.com/eureadit/crowdsourcing-ontology/master/owl/crowdsourcing-evidences.owl.ttl</hasComponent>
        <user_story>John, an individual concerned about climate change, is our user. He holds a strong belief in the reality of climate change. John comes across a set of temperature data, the temperature data is complex and contains both supportive and ambiguous information about climate change.

Within the temperature data, there is a vague statement that is not clear in its implications. John, being prone to subjective validation bias, tends to interpret ambiguous information in a way that aligns with his existing belief.

John notices a piece of information in the data that appears to support his climate change belief. Due to his subjective validation bias, he readily accepts and reinforces this confirming information. Simultaneously, there is another piece of information challenging aspects of his climate change belief within the temperature data. John, influenced by subjective validation bias, may find it difficult to accept or acknowledge this conflicting information.

As John navigates through the information, he realizes how his subjective validation bias plays a role in selectively perceiving data that aligns with his pre-existing beliefs. He becomes aware of the challenge of objectively assessing information when influenced by subjective validation bias.

John acknowledges that being aware of his own biases is essential to critically evaluate information, especially when it comes to topics like climate change. He recognizes the importance of considering diverse perspectives and interpreting data objectively. Inspired by his newfound awareness, John decides to actively seek out information that challenges his beliefs about climate change.

Through this exploration, John gains insights into his own cognitive biases and the impact of subjective validation on his beliefs. He becomes more conscious of the need to approach information with an open mind, considering both confirming and challenging aspects.</user_story>
        <rdfs:comment>Subjective Validation, also known as the personal validation effect, is a cognitive bias where people consider a statement or another piece of information to be correct if it has any personal meaning or significance to them¹². In other words, individuals are more likely to believe or accept an idea or statement if it presents to them in a personal and positive way¹.

This bias often leads people to perceive two unrelated events to be related because their personal beliefs demand that they be related¹. It&apos;s closely related to the Forer effect and is an important element in cold reading¹. Subjective validation is considered to be the main reason behind most reports of paranormal phenomena¹.

An example of subjective validation can be found in horoscopes, which often make vague, easily generalized personal statements, sometimes referred to as &quot;Barnum statements&quot;, designed to apply to nearly any individual¹. This can cause one to attribute future success to the horoscope and feel as if their belief in it has been validated¹.

In essence, subjective validation is a confirmation bias towards information that personally benefits one&apos;s self-esteem¹. Many of the validations that are given are not necessarily because they are true about recipients but because people wish it was true about themselves¹. This effect can be seen when it comes to health. For example, if someone enjoys eating bacon and they were to come across an article that talks about bacon being healthy, they will tend to believe it more because this &quot;validates&quot; eating more bacon¹.</rdfs:comment>
    </owl:Ontology>
    


    <!-- 
    ///////////////////////////////////////////////////////////////////////////////////////
    //
    // Annotation properties
    //
    ///////////////////////////////////////////////////////////////////////////////////////
     -->

    


    <!-- http://purl.org/dc/terms/created -->

    <owl:AnnotationProperty rdf:about="http://purl.org/dc/terms/created"/>
    


    <!-- http://purl.org/dc/terms/creator -->

    <owl:AnnotationProperty rdf:about="http://purl.org/dc/terms/creator"/>
    


    <!-- http://purl.org/dc/terms/description -->

    <owl:AnnotationProperty rdf:about="http://purl.org/dc/terms/description"/>
    


    <!-- http://purl.org/dc/terms/title -->

    <owl:AnnotationProperty rdf:about="http://purl.org/dc/terms/title"/>
    


    <!-- http://www.semanticweb.org/mguen/ontologies/2024/0/CognitiveBiasOntology/subjective_validation#hasComponent -->

    <owl:AnnotationProperty rdf:about="http://www.semanticweb.org/mguen/ontologies/2024/0/CognitiveBiasOntology/subjective_validation#hasComponent"/>
    


    <!-- http://www.semanticweb.org/mguen/ontologies/2024/0/CognitiveBiasOntology/subjective_validation#user_story -->

    <owl:AnnotationProperty rdf:about="http://www.semanticweb.org/mguen/ontologies/2024/0/CognitiveBiasOntology/subjective_validation#user_story"/>
    


    <!-- 
    ///////////////////////////////////////////////////////////////////////////////////////
    //
    // Object Properties
    //
    ///////////////////////////////////////////////////////////////////////////////////////
     -->

    


    <!-- http://etna.istc.cnr.it/framester2/conceptnet/5.7.0/c/en/challenges -->

    <owl:ObjectProperty rdf:about="http://etna.istc.cnr.it/framester2/conceptnet/5.7.0/c/en/challenges">
        <owl:inverseOf rdf:resource="http://etna.istc.cnr.it/framester2/conceptnet/5.7.0/c/en/confirms"/>
        <rdfs:domain rdf:resource="http://www.semanticweb.org/mguen/ontologies/2024/0/CognitiveBiasOntology/subjective_validation#Challenge"/>
        <rdfs:range rdf:resource="http://www.semanticweb.org/mguen/ontologies/2024/0/CognitiveBiasOntology/subjective_validation#Belief"/>
        <rdfs:comment>Links the challenge to the belief it challenges.</rdfs:comment>
    </owl:ObjectProperty>
    


    <!-- http://etna.istc.cnr.it/framester2/conceptnet/5.7.0/c/en/confirms -->

    <owl:ObjectProperty rdf:about="http://etna.istc.cnr.it/framester2/conceptnet/5.7.0/c/en/confirms">
        <rdfs:domain rdf:resource="http://www.semanticweb.org/mguen/ontologies/2024/0/CognitiveBiasOntology/subjective_validation#Confirmation"/>
        <rdfs:range rdf:resource="http://www.semanticweb.org/mguen/ontologies/2024/0/CognitiveBiasOntology/subjective_validation#Belief"/>
        <rdfs:comment>Links the confirmation to the belief it supports.</rdfs:comment>
    </owl:ObjectProperty>
    


    <!-- http://krisnadhi.github.io/onto/event.owl#hasInformationObject -->

    <owl:ObjectProperty rdf:about="http://krisnadhi.github.io/onto/event.owl#hasInformationObject">
        <rdfs:domain rdf:resource="http://www.ontologydesignpatterns.org/ont/dul/DUL.owl#SocialAgent"/>
        <rdfs:range rdf:resource="http://krisnadhi.github.io/onto/event.owl#InformationObject"/>
        <rdfs:comment>Links the actor to the information they encounter.</rdfs:comment>
    </owl:ObjectProperty>
    


    <!-- http://www.ontology.se/odp/content/owl/Action.owl#has_consequence -->

    <owl:ObjectProperty rdf:about="http://www.ontology.se/odp/content/owl/Action.owl#has_consequence">
        <rdfs:domain rdf:resource="http://www.ontology.se/odp/content/owl/Action.owl#Action"/>
        <rdfs:range rdf:resource="http://www.semanticweb.org/mguen/ontologies/2024/0/CognitiveBiasOntology/subjective_validation#BehavioralOutcome"/>
        <rdfs:comment>(owl:TransitiveProperty) A causal relation between actions, i.e. one action is the cause of another action. For example, the action of &quot;swimming&quot; is a consequence of &quot;jumping into deep water&quot;. The property is transitive.</rdfs:comment>
    </owl:ObjectProperty>
    


    <!-- http://www.semanticweb.org/mguen/ontologies/2024/0/CognitiveBiasOntology/subjective_validation#holds -->

    <owl:ObjectProperty rdf:about="http://www.semanticweb.org/mguen/ontologies/2024/0/CognitiveBiasOntology/subjective_validation#holds">
        <rdfs:domain rdf:resource="http://www.ontologydesignpatterns.org/ont/dul/DUL.owl#SocialAgent"/>
        <rdfs:range rdf:resource="http://www.semanticweb.org/mguen/ontologies/2024/0/CognitiveBiasOntology/subjective_validation#Belief"/>
        <rdfs:comment>Links the social agent to the belief they hold.</rdfs:comment>
    </owl:ObjectProperty>
    


    <!-- http://www.semanticweb.org/mguen/ontologies/2024/0/CognitiveBiasOntology/subjective_validation#influences -->

    <owl:ObjectProperty rdf:about="http://www.semanticweb.org/mguen/ontologies/2024/0/CognitiveBiasOntology/subjective_validation#influences">
        <rdfs:domain rdf:resource="http://www.semanticweb.org/mguen/ontologies/2024/0/CognitiveBiasOntology/subjective_validation#Belief"/>
        <rdfs:range rdf:resource="http://www.ontology.se/odp/content/owl/Action.owl#Action"/>
    </owl:ObjectProperty>
    


    <!-- http://www.semanticweb.org/mguen/ontologies/2024/0/CognitiveBiasOntology/subjective_validation#interpret -->

    <owl:ObjectProperty rdf:about="http://www.semanticweb.org/mguen/ontologies/2024/0/CognitiveBiasOntology/subjective_validation#interpret">
        <rdfs:domain rdf:resource="http://www.ontologydesignpatterns.org/ont/dul/DUL.owl#SocialAgent"/>
        <rdfs:range rdf:resource="http://www.semanticweb.org/mguen/ontologies/2024/0/CognitiveBiasOntology/subjective_validation#Statement"/>
        <rdfs:comment>Links the actor to the statement they interpret.</rdfs:comment>
    </owl:ObjectProperty>
    


    <!-- http://www.semanticweb.org/mguen/ontologies/2024/0/CognitiveBiasOntology/subjective_validation#providesInformation -->

    <owl:ObjectProperty rdf:about="http://www.semanticweb.org/mguen/ontologies/2024/0/CognitiveBiasOntology/subjective_validation#providesInformation">
        <rdfs:domain rdf:resource="http://www.semanticweb.org/mguen/ontologies/2024/0/CognitiveBiasOntology/subjective_validation#Statement"/>
        <rdfs:range rdf:resource="http://www.semanticweb.org/mguen/ontologies/2024/0/CognitiveBiasOntology/subjective_validation#Belief"/>
        <rdfs:comment>Relates an Information to a Belief. The information that can be ambiguous strongly influences the beliefe</rdfs:comment>
    </owl:ObjectProperty>
    


    <!-- http://www.semanticweb.org/mguen/ontologies/2024/0/CognitiveBiasOntology/subjective_validation#takesAction -->

    <owl:ObjectProperty rdf:about="http://www.semanticweb.org/mguen/ontologies/2024/0/CognitiveBiasOntology/subjective_validation#takesAction">
        <rdfs:domain rdf:resource="http://www.ontologydesignpatterns.org/ont/dul/DUL.owl#SocialAgent"/>
        <rdfs:range rdf:resource="http://www.ontology.se/odp/content/owl/Action.owl#Action"/>
        <rdfs:comment>Links the actor to the action they take.</rdfs:comment>
    </owl:ObjectProperty>
    


    <!-- 
    ///////////////////////////////////////////////////////////////////////////////////////
    //
    // Data properties
    //
    ///////////////////////////////////////////////////////////////////////////////////////
     -->

    


    <!-- http://www.semanticweb.org/mguen/ontologies/2024/0/CognitiveBiasOntology/subjective_validation#hasAmbiguity -->

    <owl:DatatypeProperty rdf:about="http://www.semanticweb.org/mguen/ontologies/2024/0/CognitiveBiasOntology/subjective_validation#hasAmbiguity">
        <rdfs:domain rdf:resource="http://www.semanticweb.org/mguen/ontologies/2024/0/CognitiveBiasOntology/subjective_validation#Statement"/>
        <rdfs:range rdf:resource="http://www.w3.org/2001/XMLSchema#boolean"/>
        <rdfs:comment>Indicates whether the statement has ambiguity</rdfs:comment>
    </owl:DatatypeProperty>
    


    <!-- http://www.semanticweb.org/mguen/ontologies/2024/0/CognitiveBiasOntology/subjective_validation#hasChallenge -->

    <owl:DatatypeProperty rdf:about="http://www.semanticweb.org/mguen/ontologies/2024/0/CognitiveBiasOntology/subjective_validation#hasChallenge">
        <rdfs:domain rdf:resource="http://www.semanticweb.org/mguen/ontologies/2024/0/CognitiveBiasOntology/subjective_validation#Challenge"/>
        <rdfs:range rdf:resource="http://www.w3.org/2001/XMLSchema#boolean"/>
        <rdfs:comment>Indicates whether the challenge is actually challenging.</rdfs:comment>
    </owl:DatatypeProperty>
    


    <!-- http://www.semanticweb.org/mguen/ontologies/2024/0/CognitiveBiasOntology/subjective_validation#hasComplexity -->

    <owl:DatatypeProperty rdf:about="http://www.semanticweb.org/mguen/ontologies/2024/0/CognitiveBiasOntology/subjective_validation#hasComplexity">
        <rdfs:domain rdf:resource="http://krisnadhi.github.io/onto/event.owl#InformationObject"/>
        <rdfs:range rdf:resource="http://www.w3.org/2001/XMLSchema#boolean"/>
        <rdfs:comment>Indicates whether the information has complexity</rdfs:comment>
    </owl:DatatypeProperty>
    


    <!-- http://www.semanticweb.org/mguen/ontologies/2024/0/CognitiveBiasOntology/subjective_validation#hasSupport -->

    <owl:DatatypeProperty rdf:about="http://www.semanticweb.org/mguen/ontologies/2024/0/CognitiveBiasOntology/subjective_validation#hasSupport">
        <rdfs:domain rdf:resource="http://www.semanticweb.org/mguen/ontologies/2024/0/CognitiveBiasOntology/subjective_validation#Confirmation"/>
        <rdfs:range rdf:resource="http://www.w3.org/2001/XMLSchema#boolean"/>
        <rdfs:comment>Indicates whether the confirmation has support</rdfs:comment>
    </owl:DatatypeProperty>
    


    <!-- 
    ///////////////////////////////////////////////////////////////////////////////////////
    //
    // Classes
    //
    ///////////////////////////////////////////////////////////////////////////////////////
     -->

    


    <!-- http://krisnadhi.github.io/onto/event.owl#InformationObject -->

    <owl:Class rdf:about="http://krisnadhi.github.io/onto/event.owl#InformationObject">
        <rdfs:comment>An entity that encapsulates all descriptive or non-defining information of the corresponding event, e.g., names, additional identifiers, textual descriptions, etc. Should normally be aligned to a separate Information Object pattern</rdfs:comment>
        <rdfs:comment>This classes represent the general knowledge the Social Agent has about the topic.</rdfs:comment>
    </owl:Class>
    


    <!-- http://www.ontology.se/odp/content/owl/Action.owl#Action -->

    <owl:Class rdf:about="http://www.ontology.se/odp/content/owl/Action.owl#Action">
        <rdfs:comment>(owl:Class) The process of doing something. An action is performed by an agent. An action can be proposed (proposed actions make up a plan), implemented or abandoned, and it has a status and possibly one or more suspension periods. Actions can have consequences and can be dependent on other actions, e.g. the action of pouring water from a cup is dependent on the action to first fill the cup with water.</rdfs:comment>
        <rdfs:comment>Represents an action taken by the actor</rdfs:comment>
    </owl:Class>
    


    <!-- http://www.ontologydesignpatterns.org/ont/dul/DUL.owl#SocialAgent -->

    <owl:Class rdf:about="http://www.ontologydesignpatterns.org/ont/dul/DUL.owl#SocialAgent">
        <owl:equivalentClass>
            <owl:Class>
                <owl:intersectionOf rdf:parseType="Collection">
                    <owl:Restriction>
                        <owl:onProperty rdf:resource="http://krisnadhi.github.io/onto/event.owl#hasInformationObject"/>
                        <owl:someValuesFrom>
                            <owl:Class>
                                <owl:intersectionOf rdf:parseType="Collection">
                                    <rdf:Description rdf:about="http://krisnadhi.github.io/onto/event.owl#InformationObject"/>
                                    <owl:Restriction>
                                        <owl:onProperty rdf:resource="http://www.semanticweb.org/mguen/ontologies/2024/0/CognitiveBiasOntology/subjective_validation#hasComplexity"/>
                                        <owl:hasValue rdf:datatype="http://www.w3.org/2001/XMLSchema#boolean">true</owl:hasValue>
                                    </owl:Restriction>
                                </owl:intersectionOf>
                            </owl:Class>
                        </owl:someValuesFrom>
                    </owl:Restriction>
                    <owl:Restriction>
                        <owl:onProperty rdf:resource="http://www.semanticweb.org/mguen/ontologies/2024/0/CognitiveBiasOntology/subjective_validation#holds"/>
                        <owl:someValuesFrom rdf:resource="http://www.semanticweb.org/mguen/ontologies/2024/0/CognitiveBiasOntology/subjective_validation#Belief"/>
                    </owl:Restriction>
                </owl:intersectionOf>
            </owl:Class>
        </owl:equivalentClass>
        <owl:equivalentClass>
            <owl:Class>
                <owl:intersectionOf rdf:parseType="Collection">
                    <owl:Restriction>
                        <owl:onProperty rdf:resource="http://www.semanticweb.org/mguen/ontologies/2024/0/CognitiveBiasOntology/subjective_validation#holds"/>
                        <owl:someValuesFrom>
                            <owl:Class>
                                <owl:intersectionOf rdf:parseType="Collection">
                                    <rdf:Description rdf:about="http://www.semanticweb.org/mguen/ontologies/2024/0/CognitiveBiasOntology/subjective_validation#Belief"/>
                                    <owl:Restriction>
                                        <owl:onProperty rdf:resource="http://www.semanticweb.org/mguen/ontologies/2024/0/CognitiveBiasOntology/subjective_validation#hasSupport"/>
                                        <owl:hasValue rdf:datatype="http://www.w3.org/2001/XMLSchema#boolean">true</owl:hasValue>
                                    </owl:Restriction>
                                </owl:intersectionOf>
                            </owl:Class>
                        </owl:someValuesFrom>
                    </owl:Restriction>
                    <owl:Restriction>
                        <owl:onProperty rdf:resource="http://www.semanticweb.org/mguen/ontologies/2024/0/CognitiveBiasOntology/subjective_validation#takesAction"/>
                        <owl:someValuesFrom rdf:resource="http://www.ontology.se/odp/content/owl/Action.owl#Action"/>
                    </owl:Restriction>
                </owl:intersectionOf>
            </owl:Class>
        </owl:equivalentClass>
        <rdfs:comment>(owl:Class) Any individual whose existence is granted simply by its social communicability and capability of action (through some PhysicalAgent)</rdfs:comment>
        <rdfs:comment>Represents a person who experiences subjective validation.</rdfs:comment>
        <rdfs:comment>a SocialAgent (John) holds some Belief and is related to an InformationObject that is complex. This could represent the scenario where John, who holds a belief about climate change, comes across complex temperature data.</rdfs:comment>
        <rdfs:comment>a SocialAgent (John) takes some Action and holds a Belief that has a support value of true. This could represent the scenario where John, who holds a supportive belief about climate change, decides to take action.</rdfs:comment>
    </owl:Class>
    


    <!-- http://www.semanticweb.org/mguen/ontologies/2024/0/CognitiveBiasOntology/subjective_validation#BehavioralOutcome -->

    <owl:Class rdf:about="http://www.semanticweb.org/mguen/ontologies/2024/0/CognitiveBiasOntology/subjective_validation#BehavioralOutcome">
        <rdfs:subClassOf rdf:resource="https://raw.githubusercontent.com/eureadit/crowdsourcing-ontology/master/owl/crowdsourcing-evidences.owl.ttl#Observation"/>
        <rdfs:comment>Represents the behavioral changes in thoughts or actions resulting from subjective validation in a particular context.</rdfs:comment>
    </owl:Class>
    


    <!-- http://www.semanticweb.org/mguen/ontologies/2024/0/CognitiveBiasOntology/subjective_validation#Belief -->

    <owl:Class rdf:about="http://www.semanticweb.org/mguen/ontologies/2024/0/CognitiveBiasOntology/subjective_validation#Belief">
        <rdfs:comment>The bielief in which affects the Social Agent</rdfs:comment>
    </owl:Class>
    


    <!-- http://www.semanticweb.org/mguen/ontologies/2024/0/CognitiveBiasOntology/subjective_validation#Challenge -->

    <owl:Class rdf:about="http://www.semanticweb.org/mguen/ontologies/2024/0/CognitiveBiasOntology/subjective_validation#Challenge">
        <owl:equivalentClass>
            <owl:Class>
                <owl:intersectionOf rdf:parseType="Collection">
                    <owl:Restriction>
                        <owl:onProperty rdf:resource="http://krisnadhi.github.io/onto/event.owl#hasInformationObject"/>
                        <owl:someValuesFrom>
                            <owl:Class>
                                <owl:intersectionOf rdf:parseType="Collection">
                                    <rdf:Description rdf:about="http://krisnadhi.github.io/onto/event.owl#InformationObject"/>
                                    <owl:Restriction>
                                        <owl:onProperty rdf:resource="http://www.semanticweb.org/mguen/ontologies/2024/0/CognitiveBiasOntology/subjective_validation#hasComplexity"/>
                                        <owl:hasValue rdf:datatype="http://www.w3.org/2001/XMLSchema#boolean">true</owl:hasValue>
                                    </owl:Restriction>
                                </owl:intersectionOf>
                            </owl:Class>
                        </owl:someValuesFrom>
                    </owl:Restriction>
                    <owl:Restriction>
                        <owl:onProperty rdf:resource="http://www.semanticweb.org/mguen/ontologies/2024/0/CognitiveBiasOntology/subjective_validation#holds"/>
                        <owl:someValuesFrom rdf:resource="http://www.semanticweb.org/mguen/ontologies/2024/0/CognitiveBiasOntology/subjective_validation#Belief"/>
                    </owl:Restriction>
                    <owl:Restriction>
                        <owl:onProperty rdf:resource="http://www.semanticweb.org/mguen/ontologies/2024/0/CognitiveBiasOntology/subjective_validation#hasChallenge"/>
                        <owl:hasValue rdf:datatype="http://www.w3.org/2001/XMLSchema#boolean">true</owl:hasValue>
                    </owl:Restriction>
                </owl:intersectionOf>
            </owl:Class>
        </owl:equivalentClass>
        <rdfs:subClassOf rdf:resource="http://www.semanticweb.org/mguen/ontologies/2024/0/CognitiveBiasOntology/subjective_validation#Statement"/>
        <rdfs:comment>Represents the act of perceiving information as opposing or challenging a belief.</rdfs:comment>
        <rdfs:comment>a Challenge is considered challenging (hasChallenge value true) if it is related to an InformationObject that is complex (hasComplexity value true) and is perceived by a SocialAgent who holds a Belief. This could represent the scenario where John perceives challenging information within complex temperature data that opposes his belief about climate change.</rdfs:comment>
    </owl:Class>
    


    <!-- http://www.semanticweb.org/mguen/ontologies/2024/0/CognitiveBiasOntology/subjective_validation#Confirmation -->

    <owl:Class rdf:about="http://www.semanticweb.org/mguen/ontologies/2024/0/CognitiveBiasOntology/subjective_validation#Confirmation">
        <owl:equivalentClass>
            <owl:Class>
                <owl:intersectionOf rdf:parseType="Collection">
                    <owl:Restriction>
                        <owl:onProperty rdf:resource="http://krisnadhi.github.io/onto/event.owl#hasInformationObject"/>
                        <owl:someValuesFrom>
                            <owl:Class>
                                <owl:intersectionOf rdf:parseType="Collection">
                                    <rdf:Description rdf:about="http://krisnadhi.github.io/onto/event.owl#InformationObject"/>
                                    <owl:Restriction>
                                        <owl:onProperty rdf:resource="http://www.semanticweb.org/mguen/ontologies/2024/0/CognitiveBiasOntology/subjective_validation#hasComplexity"/>
                                        <owl:hasValue rdf:datatype="http://www.w3.org/2001/XMLSchema#boolean">true</owl:hasValue>
                                    </owl:Restriction>
                                </owl:intersectionOf>
                            </owl:Class>
                        </owl:someValuesFrom>
                    </owl:Restriction>
                    <owl:Restriction>
                        <owl:onProperty rdf:resource="http://www.semanticweb.org/mguen/ontologies/2024/0/CognitiveBiasOntology/subjective_validation#holds"/>
                        <owl:someValuesFrom rdf:resource="http://www.semanticweb.org/mguen/ontologies/2024/0/CognitiveBiasOntology/subjective_validation#Belief"/>
                    </owl:Restriction>
                    <owl:Restriction>
                        <owl:onProperty rdf:resource="http://www.semanticweb.org/mguen/ontologies/2024/0/CognitiveBiasOntology/subjective_validation#hasSupport"/>
                        <owl:hasValue rdf:datatype="http://www.w3.org/2001/XMLSchema#boolean">true</owl:hasValue>
                    </owl:Restriction>
                </owl:intersectionOf>
            </owl:Class>
        </owl:equivalentClass>
        <rdfs:subClassOf rdf:resource="http://www.semanticweb.org/mguen/ontologies/2024/0/CognitiveBiasOntology/subjective_validation#Statement"/>
        <rdfs:comment>Represents the act of perceiving information as supporting or confirming a belief.</rdfs:comment>
        <rdfs:comment>a Confirmation is considered supportive (hasSupport value true) if it is related to an InformationObject that is complex (hasComplexity value true) and is perceived by a SocialAgent who holds a Belief. This could represent the scenario where John perceives supportive information within complex temperature data that confirms his belief about climate change.</rdfs:comment>
    </owl:Class>
    


    <!-- http://www.semanticweb.org/mguen/ontologies/2024/0/CognitiveBiasOntology/subjective_validation#Statement -->

    <owl:Class rdf:about="http://www.semanticweb.org/mguen/ontologies/2024/0/CognitiveBiasOntology/subjective_validation#Statement">
        <owl:equivalentClass>
            <owl:Class>
                <owl:intersectionOf rdf:parseType="Collection">
                    <owl:Restriction>
                        <owl:onProperty rdf:resource="http://krisnadhi.github.io/onto/event.owl#hasInformationObject"/>
                        <owl:someValuesFrom>
                            <owl:Class>
                                <owl:intersectionOf rdf:parseType="Collection">
                                    <rdf:Description rdf:about="http://krisnadhi.github.io/onto/event.owl#InformationObject"/>
                                    <owl:Restriction>
                                        <owl:onProperty rdf:resource="http://www.semanticweb.org/mguen/ontologies/2024/0/CognitiveBiasOntology/subjective_validation#hasComplexity"/>
                                        <owl:hasValue rdf:datatype="http://www.w3.org/2001/XMLSchema#boolean">true</owl:hasValue>
                                    </owl:Restriction>
                                </owl:intersectionOf>
                            </owl:Class>
                        </owl:someValuesFrom>
                    </owl:Restriction>
                    <owl:Restriction>
                        <owl:onProperty rdf:resource="http://www.semanticweb.org/mguen/ontologies/2024/0/CognitiveBiasOntology/subjective_validation#hasAmbiguity"/>
                        <owl:hasValue rdf:datatype="http://www.w3.org/2001/XMLSchema#boolean">true</owl:hasValue>
                    </owl:Restriction>
                </owl:intersectionOf>
            </owl:Class>
        </owl:equivalentClass>
        <rdfs:subClassOf rdf:resource="http://krisnadhi.github.io/onto/event.owl#InformationObject"/>
        <rdfs:comment>Represents a specific piece of information or claim that can be ambiguous or not.</rdfs:comment>
        <rdfs:comment>a Statement is considered ambiguous (hasAmbiguity value true) if it is related to an InformationObject that is complex (hasComplexity value true). This could represent the scenario where John interprets a specific piece of information or claim within the complex temperature data that can be ambiguous.</rdfs:comment>
    </owl:Class>
    


    <!-- https://raw.githubusercontent.com/eureadit/crowdsourcing-ontology/master/owl/crowdsourcing-evidences.owl.ttl#Observation -->

    <owl:Class rdf:about="https://raw.githubusercontent.com/eureadit/crowdsourcing-ontology/master/owl/crowdsourcing-evidences.owl.ttl#Observation">
        <rdfs:comment>(owl:Class) The product of an act of scrutiny which may or may not have been performed with a critical disposition (Example: &quot;My thoughts from reading this passage of &apos;To Kill a Mockingbird&apos;&quot;).</rdfs:comment>
    </owl:Class>
    


    <!-- 
    ///////////////////////////////////////////////////////////////////////////////////////
    //
    // Individuals
    //
    ///////////////////////////////////////////////////////////////////////////////////////
     -->

    


    <!-- http://www.semanticweb.org/mguen/ontologies/2024/0/CognitiveBiasOntology/subjective_validation#DecisionToSeekChallengingInfo -->

    <owl:NamedIndividual rdf:about="http://www.semanticweb.org/mguen/ontologies/2024/0/CognitiveBiasOntology/subjective_validation#DecisionToSeekChallengingInfo">
        <rdf:type rdf:resource="http://www.semanticweb.org/mguen/ontologies/2024/0/CognitiveBiasOntology/subjective_validation#BehavioralOutcome"/>
    </owl:NamedIndividual>
    


    <!-- http://www.semanticweb.org/mguen/ontologies/2024/0/CognitiveBiasOntology/subjective_validation#InfoChallengingJohnBelief -->

    <owl:NamedIndividual rdf:about="http://www.semanticweb.org/mguen/ontologies/2024/0/CognitiveBiasOntology/subjective_validation#InfoChallengingJohnBelief">
        <rdf:type rdf:resource="http://www.semanticweb.org/mguen/ontologies/2024/0/CognitiveBiasOntology/subjective_validation#Challenge"/>
    </owl:NamedIndividual>
    


    <!-- http://www.semanticweb.org/mguen/ontologies/2024/0/CognitiveBiasOntology/subjective_validation#InfoSupportingJohnBelief -->

    <owl:NamedIndividual rdf:about="http://www.semanticweb.org/mguen/ontologies/2024/0/CognitiveBiasOntology/subjective_validation#InfoSupportingJohnBelief">
        <rdf:type rdf:resource="http://www.semanticweb.org/mguen/ontologies/2024/0/CognitiveBiasOntology/subjective_validation#Confirmation"/>
    </owl:NamedIndividual>
    


    <!-- http://www.semanticweb.org/mguen/ontologies/2024/0/CognitiveBiasOntology/subjective_validation#John -->

    <owl:NamedIndividual rdf:about="http://www.semanticweb.org/mguen/ontologies/2024/0/CognitiveBiasOntology/subjective_validation#John">
        <rdf:type rdf:resource="http://www.ontologydesignpatterns.org/ont/dul/DUL.owl#SocialAgent"/>
    </owl:NamedIndividual>
    


    <!-- http://www.semanticweb.org/mguen/ontologies/2024/0/CognitiveBiasOntology/subjective_validation#NavigatingTroughInfo -->

    <owl:NamedIndividual rdf:about="http://www.semanticweb.org/mguen/ontologies/2024/0/CognitiveBiasOntology/subjective_validation#NavigatingTroughInfo">
        <rdf:type rdf:resource="http://www.ontology.se/odp/content/owl/Action.owl#Action"/>
    </owl:NamedIndividual>
    


    <!-- http://www.semanticweb.org/mguen/ontologies/2024/0/CognitiveBiasOntology/subjective_validation#TemperatureData -->

    <owl:NamedIndividual rdf:about="http://www.semanticweb.org/mguen/ontologies/2024/0/CognitiveBiasOntology/subjective_validation#TemperatureData">
        <rdf:type rdf:resource="http://krisnadhi.github.io/onto/event.owl#InformationObject"/>
    </owl:NamedIndividual>
    


    <!-- http://www.semanticweb.org/mguen/ontologies/2024/0/CognitiveBiasOntology/subjective_validation#VagueStatement -->

    <owl:NamedIndividual rdf:about="http://www.semanticweb.org/mguen/ontologies/2024/0/CognitiveBiasOntology/subjective_validation#VagueStatement">
        <rdf:type rdf:resource="http://www.semanticweb.org/mguen/ontologies/2024/0/CognitiveBiasOntology/subjective_validation#Statement"/>
    </owl:NamedIndividual>
    


    <!-- http://www.semanticweb.org/mguen/ontologies/2024/0/CognitiveBiasOntology/subjective_validation#John&apos;sBelief -->

    <owl:NamedIndividual rdf:about="http://www.semanticweb.org/mguen/ontologies/2024/0/CognitiveBiasOntology/subjective_validation#John&apos;sBelief">
        <rdf:type rdf:resource="http://www.semanticweb.org/mguen/ontologies/2024/0/CognitiveBiasOntology/subjective_validation#Belief"/>
    </owl:NamedIndividual>
</rdf:RDF>



<!-- Generated by the OWL API (version 4.5.25.2023-02-15T19:15:49Z) https://github.com/owlcs/owlapi -->

