<?xml version="1.0"?>
<rdf:RDF xmlns="http://www.semanticweb.org/lucia/ontologies/2024/0/testing_effect#"
     xml:base="http://www.semanticweb.org/lucia/ontologies/2024/0/testing_effect"
     xmlns:cbo="http://www.semanticweb.org/lucia/ontologies/2024/0/CognitiveBiasOntology/testing_effect/"
     xmlns:owl="http://www.w3.org/2002/07/owl#"
     xmlns:rdf="http://www.w3.org/1999/02/22-rdf-syntax-ns#"
     xmlns:xml="http://www.w3.org/XML/1998/namespace"
     xmlns:xsd="http://www.w3.org/2001/XMLSchema#"
     xmlns:rdfs="http://www.w3.org/2000/01/rdf-schema#">
    <owl:Ontology rdf:about="http://www.semanticweb.org/lucia/ontologies/2024/0/testing_effect">
        <rdfs:comment>This is an ontology of the cognitive bias of the testing effect</rdfs:comment>
    </owl:Ontology>
    


    <!-- 
    ///////////////////////////////////////////////////////////////////////////////////////
    //
    // Object Properties
    //
    ///////////////////////////////////////////////////////////////////////////////////////
     -->

    


    <!-- http://www.semanticweb.org/lucia/ontologies/2024/0/testing_effect#EnhancesRetention -->

    <owl:ObjectProperty rdf:about="http://www.semanticweb.org/lucia/ontologies/2024/0/testing_effect#EnhancesRetention">
        <rdfs:domain rdf:resource="http://www.semanticweb.org/lucia/ontologies/2024/0/testing_effect#TestingEvent"/>
        <rdfs:range rdf:resource="http://www.semanticweb.org/lucia/ontologies/2024/0/testing_effect#LearningMaterial"/>
        <rdfs:comment>Represents the impact of actively recalling information on long-term retention, connecting an Individual to a TestingEvent</rdfs:comment>
    </owl:ObjectProperty>
    


    <!-- http://www.semanticweb.org/lucia/ontologies/2024/0/testing_effect#engagesInLearning -->

    <owl:ObjectProperty rdf:about="http://www.semanticweb.org/lucia/ontologies/2024/0/testing_effect#engagesInLearning">
        <rdfs:domain rdf:resource="http://www.semanticweb.org/lucia/ontologies/2024/0/testing_effect#Individual"/>
        <rdfs:range rdf:resource="http://www.semanticweb.org/lucia/ontologies/2024/0/testing_effect#LearningProcess"/>
        <rdfs:comment>Relates an Individual to the concept of actively participating in a learning process</rdfs:comment>
    </owl:ObjectProperty>
    


    <!-- http://www.semanticweb.org/lucia/ontologies/2024/0/testing_effect#participatesInTesting -->

    <owl:ObjectProperty rdf:about="http://www.semanticweb.org/lucia/ontologies/2024/0/testing_effect#participatesInTesting">
        <rdfs:domain rdf:resource="http://www.semanticweb.org/lucia/ontologies/2024/0/testing_effect#Individual"/>
        <rdfs:range rdf:resource="http://www.semanticweb.org/lucia/ontologies/2024/0/testing_effect#TestingEvent"/>
        <rdfs:comment>Relates an Individual to a TestingEvent, indicating their engagement in an active recall or testing session</rdfs:comment>
    </owl:ObjectProperty>
    


    <!-- http://www.semanticweb.org/lucia/ontologies/2024/0/testing_effect#studiesMaterial -->

    <owl:ObjectProperty rdf:about="http://www.semanticweb.org/lucia/ontologies/2024/0/testing_effect#studiesMaterial">
        <rdfs:domain rdf:resource="http://www.semanticweb.org/lucia/ontologies/2024/0/testing_effect#Individual"/>
        <rdfs:range rdf:resource="http://www.semanticweb.org/lucia/ontologies/2024/0/testing_effect#LearningMaterial"/>
        <rdfs:comment>Relates an Individual to LearningMaterial, indicating the educational content being studied</rdfs:comment>
    </owl:ObjectProperty>
    


    <!-- 
    ///////////////////////////////////////////////////////////////////////////////////////
    //
    // Classes
    //
    ///////////////////////////////////////////////////////////////////////////////////////
     -->

    


    <!-- http://www.semanticweb.org/lucia/ontologies/2024/0/testing_effect#Individual -->

    <owl:Class rdf:about="http://www.semanticweb.org/lucia/ontologies/2024/0/testing_effect#Individual">
        <rdfs:comment>Represents a person participating in a group activity</rdfs:comment>
    </owl:Class>
    


    <!-- http://www.semanticweb.org/lucia/ontologies/2024/0/testing_effect#LearningMaterial -->

    <owl:Class rdf:about="http://www.semanticweb.org/lucia/ontologies/2024/0/testing_effect#LearningMaterial">
        <rdfs:comment>Represents the educational content or material being studied</rdfs:comment>
    </owl:Class>
    


    <!-- http://www.semanticweb.org/lucia/ontologies/2024/0/testing_effect#LearningProcess -->

    <owl:Class rdf:about="http://www.semanticweb.org/lucia/ontologies/2024/0/testing_effect#LearningProcess">
        <rdfs:comment>The process of learning the an individual undertakes in order to memorise the learning material</rdfs:comment>
    </owl:Class>
    


    <!-- http://www.semanticweb.org/lucia/ontologies/2024/0/testing_effect#TestingEvent -->

    <owl:Class rdf:about="http://www.semanticweb.org/lucia/ontologies/2024/0/testing_effect#TestingEvent">
        <rdfs:subClassOf>
            <owl:Restriction>
                <owl:onProperty rdf:resource="http://www.semanticweb.org/lucia/ontologies/2024/0/testing_effect#EnhancesRetention"/>
                <owl:someValuesFrom rdf:resource="http://www.semanticweb.org/lucia/ontologies/2024/0/testing_effect#LearningMaterial"/>
            </owl:Restriction>
        </rdfs:subClassOf>
        <rdfs:comment>Represents an instance of actively recalling information through testing or self-assessment</rdfs:comment>
    </owl:Class>
</rdf:RDF>



<!-- Generated by the OWL API (version 4.5.25.2023-02-15T19:15:49Z) https://github.com/owlcs/owlapi -->

