<?xml version="1.0"?>
<rdf:RDF xmlns="http://www.semanticweb.org/mguen/ontologies/2024/1/CognitiveBiasOntology/tip_of_the_tongue_phenomenon#"
     xml:base="http://www.semanticweb.org/mguen/ontologies/2024/1/CognitiveBiasOntology/tip_of_the_tongue_phenomenon"
     xmlns:cbo="http://www.semanticweb.org/mguen/ontologies/2024/1/CognitiveBiasOntology/tip_of_the_tongue_phenomenon/"
     xmlns:owl="http://www.w3.org/2002/07/owl#"
     xmlns:rdf="http://www.w3.org/1999/02/22-rdf-syntax-ns#"
     xmlns:xml="http://www.w3.org/XML/1998/namespace"
     xmlns:xsd="http://www.w3.org/2001/XMLSchema#"
     xmlns:rdfs="http://www.w3.org/2000/01/rdf-schema#">
    <owl:Ontology rdf:about="http://www.semanticweb.org/mguen/ontologies/2024/1/CognitiveBiasOntology/tip_of_the_tongue_phenomenon"/>
    


    <!-- 
    ///////////////////////////////////////////////////////////////////////////////////////
    //
    // Object Properties
    //
    ///////////////////////////////////////////////////////////////////////////////////////
     -->

    


    <!-- http://www.semanticweb.org/mguen/ontologies/2024/1/CognitiveBiasOntology/tip_of_the_tongue_phenomenon#experiencesEmotion -->

    <owl:ObjectProperty rdf:about="http://www.semanticweb.org/mguen/ontologies/2024/1/CognitiveBiasOntology/tip_of_the_tongue_phenomenon#experiencesEmotion">
        <rdfs:domain rdf:resource="http://etna.istc.cnr.it/framester2/conceptnet/5.7.0/c/en/individual"/>
        <rdfs:range rdf:resource="http://www.semanticweb.org/mguen/ontologies/2024/1/CognitiveBiasOntology/tip_of_the_tongue_phenomenon#CognitiveProcess"/>
        <rdfs:comment>Relates an individual to the cognitive processes involved in memory retrieval during the Tip of the Tongue phenomenon.</rdfs:comment>
    </owl:ObjectProperty>
    


    <!-- http://www.semanticweb.org/mguen/ontologies/2024/1/CognitiveBiasOntology/tip_of_the_tongue_phenomenon#hasPartialInformation -->

    <owl:ObjectProperty rdf:about="http://www.semanticweb.org/mguen/ontologies/2024/1/CognitiveBiasOntology/tip_of_the_tongue_phenomenon#hasPartialInformation">
        <rdfs:domain rdf:resource="http://etna.istc.cnr.it/framester2/conceptnet/5.7.0/c/en/individual"/>
        <rdfs:range rdf:resource="http://www.semanticweb.org/mguen/ontologies/2024/1/CognitiveBiasOntology/tip_of_the_tongue_phenomenon#PartialInformation"/>
        <rdfs:comment>Relates an individual to the bits of information they can recall about the target word during the Tip of the Tongue phenomenon.</rdfs:comment>
    </owl:ObjectProperty>
    


    <!-- http://www.semanticweb.org/mguen/ontologies/2024/1/CognitiveBiasOntology/tip_of_the_tongue_phenomenon#leavesMemoryTrace -->

    <owl:ObjectProperty rdf:about="http://www.semanticweb.org/mguen/ontologies/2024/1/CognitiveBiasOntology/tip_of_the_tongue_phenomenon#leavesMemoryTrace">
        <rdfs:domain rdf:resource="http://www.semanticweb.org/mguen/ontologies/2024/1/CognitiveBiasOntology/tip_of_the_tongue_phenomenon#CognitiveProcess"/>
        <rdfs:range rdf:resource="http://www.semanticweb.org/mguen/ontologies/2024/1/CognitiveBiasOntology/tip_of_the_tongue_phenomenon#MemoryTrace"/>
        <rdfs:comment>Relates a cognitive process to the memory trace it leaves in the brain during the Tip of the Tongue phenomenon.</rdfs:comment>
    </owl:ObjectProperty>
    


    <!-- https://en.wiktionary.org/wiki/experiences -->

    <owl:ObjectProperty rdf:about="https://en.wiktionary.org/wiki/experiences">
        <rdfs:domain rdf:resource="http://etna.istc.cnr.it/framester2/conceptnet/5.7.0/c/en/individual"/>
        <rdfs:range rdf:resource="http://www.semanticweb.org/mguen/ontologies/2024/1/CognitiveBiasOntology/tip_of_the_tongue_phenomenon#TargetWord"/>
        <rdfs:comment>Relates an individual to the specific word or piece of information they are trying to recall during the Tip of the Tongue phenomenon.</rdfs:comment>
    </owl:ObjectProperty>
    


    <!-- 
    ///////////////////////////////////////////////////////////////////////////////////////
    //
    // Classes
    //
    ///////////////////////////////////////////////////////////////////////////////////////
     -->

    


    <!-- http://etna.istc.cnr.it/framester2/conceptnet/5.7.0/c/en/individual -->

    <owl:Class rdf:about="http://etna.istc.cnr.it/framester2/conceptnet/5.7.0/c/en/individual">
        <rdfs:comment>The person experiencing the Tip of The Tongue Phenomenon.</rdfs:comment>
    </owl:Class>
    


    <!-- http://etna.istc.cnr.it/framesterpage/conceptnet/5.7.0/c/en/context -->

    <owl:Class rdf:about="http://etna.istc.cnr.it/framesterpage/conceptnet/5.7.0/c/en/context">
        <rdfs:comment>The specific situation or domain in which the Tip of The Tongue Phenomenon is being experienced.</rdfs:comment>
    </owl:Class>
    


    <!-- http://www.semanticweb.org/mguen/ontologies/2024/1/CognitiveBiasOntology/tip_of_the_tongue_phenomenon#CognitiveProcess -->

    <owl:Class rdf:about="http://www.semanticweb.org/mguen/ontologies/2024/1/CognitiveBiasOntology/tip_of_the_tongue_phenomenon#CognitiveProcess">
        <rdfs:comment>The cognitive processes involved in memory retrieval.</rdfs:comment>
    </owl:Class>
    


    <!-- http://www.semanticweb.org/mguen/ontologies/2024/1/CognitiveBiasOntology/tip_of_the_tongue_phenomenon#MemoryTrace -->

    <owl:Class rdf:about="http://www.semanticweb.org/mguen/ontologies/2024/1/CognitiveBiasOntology/tip_of_the_tongue_phenomenon#MemoryTrace">
        <rdfs:comment>The trace that a memory leaves in the brain.</rdfs:comment>
    </owl:Class>
    


    <!-- http://www.semanticweb.org/mguen/ontologies/2024/1/CognitiveBiasOntology/tip_of_the_tongue_phenomenon#PartialInformation -->

    <owl:Class rdf:about="http://www.semanticweb.org/mguen/ontologies/2024/1/CognitiveBiasOntology/tip_of_the_tongue_phenomenon#PartialInformation">
        <rdfs:comment>The bits of information about the target word that the individual can recall.</rdfs:comment>
    </owl:Class>
    


    <!-- http://www.semanticweb.org/mguen/ontologies/2024/1/CognitiveBiasOntology/tip_of_the_tongue_phenomenon#TargetWord -->

    <owl:Class rdf:about="http://www.semanticweb.org/mguen/ontologies/2024/1/CognitiveBiasOntology/tip_of_the_tongue_phenomenon#TargetWord">
        <rdfs:comment>The word or piece of information that the individual is trying to recall.</rdfs:comment>
    </owl:Class>
    


    <!-- https://dbpedia.org/Emotion -->

    <owl:Class rdf:about="https://dbpedia.org/Emotion">
        <rdfs:comment>The feelings experienced by the individual during the phenomenon.</rdfs:comment>
    </owl:Class>
    


    <!-- 
    ///////////////////////////////////////////////////////////////////////////////////////
    //
    // Individuals
    //
    ///////////////////////////////////////////////////////////////////////////////////////
     -->

    


    <!-- http://www.semanticweb.org/mguen/ontologies/2024/1/CognitiveBiasOntology/tip_of_the_tongue_phenomenon#Amanda -->

    <owl:NamedIndividual rdf:about="http://www.semanticweb.org/mguen/ontologies/2024/1/CognitiveBiasOntology/tip_of_the_tongue_phenomenon#Amanda">
        <rdf:type rdf:resource="http://etna.istc.cnr.it/framester2/conceptnet/5.7.0/c/en/individual"/>
    </owl:NamedIndividual>
    


    <!-- http://www.semanticweb.org/mguen/ontologies/2024/1/CognitiveBiasOntology/tip_of_the_tongue_phenomenon#Emily -->

    <owl:NamedIndividual rdf:about="http://www.semanticweb.org/mguen/ontologies/2024/1/CognitiveBiasOntology/tip_of_the_tongue_phenomenon#Emily">
        <rdf:type rdf:resource="http://etna.istc.cnr.it/framester2/conceptnet/5.7.0/c/en/individual"/>
    </owl:NamedIndividual>
    


    <!-- http://www.semanticweb.org/mguen/ontologies/2024/1/CognitiveBiasOntology/tip_of_the_tongue_phenomenon#Frustration -->

    <owl:NamedIndividual rdf:about="http://www.semanticweb.org/mguen/ontologies/2024/1/CognitiveBiasOntology/tip_of_the_tongue_phenomenon#Frustration">
        <rdf:type rdf:resource="https://dbpedia.org/Emotion"/>
    </owl:NamedIndividual>
    


    <!-- http://www.semanticweb.org/mguen/ontologies/2024/1/CognitiveBiasOntology/tip_of_the_tongue_phenomenon#MemoryRetrieval -->

    <owl:NamedIndividual rdf:about="http://www.semanticweb.org/mguen/ontologies/2024/1/CognitiveBiasOntology/tip_of_the_tongue_phenomenon#MemoryRetrieval">
        <rdf:type rdf:resource="http://www.semanticweb.org/mguen/ontologies/2024/1/CognitiveBiasOntology/tip_of_the_tongue_phenomenon#CognitiveProcess"/>
    </owl:NamedIndividual>
    


    <!-- http://www.semanticweb.org/mguen/ontologies/2024/1/CognitiveBiasOntology/tip_of_the_tongue_phenomenon#NetworkingEvent -->

    <owl:NamedIndividual rdf:about="http://www.semanticweb.org/mguen/ontologies/2024/1/CognitiveBiasOntology/tip_of_the_tongue_phenomenon#NetworkingEvent">
        <rdf:type rdf:resource="http://etna.istc.cnr.it/framesterpage/conceptnet/5.7.0/c/en/context"/>
    </owl:NamedIndividual>
    


    <!-- http://www.semanticweb.org/mguen/ontologies/2024/1/CognitiveBiasOntology/tip_of_the_tongue_phenomenon#RecallFailure -->

    <owl:NamedIndividual rdf:about="http://www.semanticweb.org/mguen/ontologies/2024/1/CognitiveBiasOntology/tip_of_the_tongue_phenomenon#RecallFailure">
        <rdf:type rdf:resource="http://www.semanticweb.org/mguen/ontologies/2024/1/CognitiveBiasOntology/tip_of_the_tongue_phenomenon#CognitiveProcess"/>
    </owl:NamedIndividual>
</rdf:RDF>



<!-- Generated by the OWL API (version 4.5.25.2023-02-15T19:15:49Z) https://github.com/owlcs/owlapi -->

