<?xml version="1.0"?>
<rdf:RDF xmlns="http://www.semanticweb.org/mguen/ontologies/2024/1/CognitiveBiasOntology/tip_of_the_tongue_phenomenon#"
     xml:base="http://www.semanticweb.org/mguen/ontologies/2024/1/CognitiveBiasOntology/tip_of_the_tongue_phenomenon"
     xmlns:ac="http://www.ontology.se/odp/content/owl/Action.owl"
     xmlns:ec="http://krisnadhi.github.io/onto/event.owl"
     xmlns:fs="http://etna.istc.cnr.it/framester2/data/framestercore/"
     xmlns:acf="http://www.ontologydesignpatterns.org/ont/dul/DUL.owl"
     xmlns:cbo="http://www.semanticweb.org/mguen/ontologies/2024/1/CognitiveBiasOntology/tip_of_the_tongue_phenomenon/"
     xmlns:owl="http://www.w3.org/2002/07/owl#"
     xmlns:rdf="http://www.w3.org/1999/02/22-rdf-syntax-ns#"
     xmlns:xml="http://www.w3.org/XML/1998/namespace"
     xmlns:xsd="http://www.w3.org/2001/XMLSchema#"
     xmlns:foaf="http://xmlns.com/foaf/0.1/"
     xmlns:rdfs="http://www.w3.org/2000/01/rdf-schema#"
     xmlns:event="http://krisnadhi.github.io/onto/event.owl#"
     xmlns:Action="http://www.ontology.se/odp/content/owl/Action.owl#"
     xmlns:dcterms="http://purl.org/dc/terms/"
     xmlns:dbpedia-owl="https://en.wiktionary.org/wiki/">
    <owl:Ontology rdf:about="http://www.semanticweb.org/mguen/ontologies/2024/1/CognitiveBiasOntology/tip_of_the_tongue_phenomenon">
        <dcterms:created>06/02/2024</dcterms:created>
        <dcterms:creator>Matteo Guenci</dcterms:creator>
        <dcterms:description>The Tip of The Tongue Phenomenon section of the Cognitive Bias Ontology.</dcterms:description>
        <dcterms:title>Tip of The Tongue Ontology</dcterms:title>
        <hasComponent>http://ontologydesignpatterns.org/wiki/Submissions:Action</hasComponent>
        <hasComponent>http://ontologydesignpatterns.org/wiki/Submissions:EventCore</hasComponent>
        <hasComponent>http://www.ontologydesignpatterns.org/ont/dul/DUL.owl</hasComponent>
        <hasComponent>http://xmlns.com/foaf/0.1/</hasComponent>
        <user_story>Meet Emily, a social butterfly who loves meeting new people. At a networking event, she met a woman who shared interesting insights about a project similar to Emily&apos;s work. They had a great conversation, and Emily wanted to connect with her later on LinkedIn.
A few days later, Emily decided to find the woman on LinkedIn. She remembered the woman&apos;s face, her project details, and even the color of her dress, but she couldn&apos;t recall her name. Emily knew it started with an &apos;A&apos;, and it was on the tip of her tongue, but she just couldn&apos;t retrieve it from her memory.
This is an example of the Tip of The Tongue Phenomenon. Despite having partial recall (the first letter of the name), Emily was unable to fully retrieve the name from her memory. She felt a sense of frustration as she knew that she knew the name, but just couldn&apos;t recall it at that moment.
Eventually, after some time, the name &quot;Amanda&quot; suddenly popped into Emily&apos;s mind. She felt a sense of relief and quickly searched for Amanda on LinkedIn. This experience reminded Emily of the peculiarities of human memory and how the feeling of knowing something can sometimes be just out of reach.</user_story>
        <rdfs:comment>The Tip of the Tongue (TOT) phenomenon, also known as lethologica, is a cognitive bias where an individual fails to retrieve a word or term from memory, despite having partial recall and the feeling that retrieval is imminent. People experiencing the TOT phenomenon can often recall one or more features of the target word, such as the first letter, its syllabic stress, and words similar in sound, meaning, or both sound and meaning. This phenomenon reveals that lexical access occurs in stages..</rdfs:comment>
    </owl:Ontology>
    


    <!-- 
    ///////////////////////////////////////////////////////////////////////////////////////
    //
    // Annotation properties
    //
    ///////////////////////////////////////////////////////////////////////////////////////
     -->

    


    <!-- http://purl.org/dc/terms/created -->

    <owl:AnnotationProperty rdf:about="http://purl.org/dc/terms/created"/>
    


    <!-- http://purl.org/dc/terms/creator -->

    <owl:AnnotationProperty rdf:about="http://purl.org/dc/terms/creator"/>
    


    <!-- http://purl.org/dc/terms/description -->

    <owl:AnnotationProperty rdf:about="http://purl.org/dc/terms/description"/>
    


    <!-- http://purl.org/dc/terms/title -->

    <owl:AnnotationProperty rdf:about="http://purl.org/dc/terms/title"/>
    


    <!-- http://www.semanticweb.org/mguen/ontologies/2024/1/CognitiveBiasOntology/tip_of_the_tongue_phenomenon#hasComponent -->

    <owl:AnnotationProperty rdf:about="http://www.semanticweb.org/mguen/ontologies/2024/1/CognitiveBiasOntology/tip_of_the_tongue_phenomenon#hasComponent"/>
    


    <!-- http://www.semanticweb.org/mguen/ontologies/2024/1/CognitiveBiasOntology/tip_of_the_tongue_phenomenon#user_story -->

    <owl:AnnotationProperty rdf:about="http://www.semanticweb.org/mguen/ontologies/2024/1/CognitiveBiasOntology/tip_of_the_tongue_phenomenon#user_story"/>
    


    <!-- 
    ///////////////////////////////////////////////////////////////////////////////////////
    //
    // Object Properties
    //
    ///////////////////////////////////////////////////////////////////////////////////////
     -->

    


    <!-- http://krisnadhi.github.io/onto/event.owl#hasInformationObject -->

    <owl:ObjectProperty rdf:about="http://krisnadhi.github.io/onto/event.owl#hasInformationObject">
        <rdfs:domain rdf:resource="http://www.ontologydesignpatterns.org/ont/dul/DUL.owl#SocialAgent"/>
        <rdfs:range rdf:resource="http://krisnadhi.github.io/onto/event.owl#InformationObject"/>
        <rdfs:comment>A relationship between a Person and the Information they have.</rdfs:comment>
        <rdfs:comment>Property relating Event to InformationObject in this pattern. The domain of this property is not restricted to Event since it is possible that non-event to have an information object. The range is always InformationObject since it makes no sense to have a property named hasInformationObject to point to anything other than information object.</rdfs:comment>
    </owl:ObjectProperty>
    


    <!-- http://www.ontology.se/odp/content/owl/Action.owl#has_consequence -->

    <owl:ObjectProperty rdf:about="http://www.ontology.se/odp/content/owl/Action.owl#has_consequence">
        <rdfs:domain rdf:resource="http://www.semanticweb.org/mguen/ontologies/2024/1/CognitiveBiasOntology/tip_of_the_tongue_phenomenon#RecallAttempt"/>
        <rdfs:range>
            <owl:Class>
                <owl:unionOf rdf:parseType="Collection">
                    <rdf:Description rdf:about="http://www.semanticweb.org/mguen/ontologies/2024/1/CognitiveBiasOntology/tip_of_the_tongue_phenomenon#MemoryBlock"/>
                    <rdf:Description rdf:about="http://www.semanticweb.org/mguen/ontologies/2024/1/CognitiveBiasOntology/tip_of_the_tongue_phenomenon#MemoryRetrieval"/>
                </owl:unionOf>
            </owl:Class>
        </rdfs:range>
        <rdfs:comment>(owl:TransitiveProperty) A causal relation between actions, i.e. one action is the cause of another action. For example, the action of &quot;swimming&quot; is a consequence of &quot;jumping into deep water&quot;. The property is transitive.</rdfs:comment>
    </owl:ObjectProperty>
    


    <!-- http://www.semanticweb.org/mguen/ontologies/2024/1/CognitiveBiasOntology/tip_of_the_tongue_phenomenon#attemptsRecall -->

    <owl:ObjectProperty rdf:about="http://www.semanticweb.org/mguen/ontologies/2024/1/CognitiveBiasOntology/tip_of_the_tongue_phenomenon#attemptsRecall">
        <rdfs:domain rdf:resource="http://www.ontologydesignpatterns.org/ont/dul/DUL.owl#SocialAgent"/>
        <rdfs:range rdf:resource="http://www.semanticweb.org/mguen/ontologies/2024/1/CognitiveBiasOntology/tip_of_the_tongue_phenomenon#RecallAttempt"/>
        <rdfs:comment>A relationship between a Person and a RecallAttempt they make or at least try to.</rdfs:comment>
    </owl:ObjectProperty>
    


    <!-- http://www.semanticweb.org/mguen/ontologies/2024/1/CognitiveBiasOntology/tip_of_the_tongue_phenomenon#experiences -->

    <owl:ObjectProperty rdf:about="http://www.semanticweb.org/mguen/ontologies/2024/1/CognitiveBiasOntology/tip_of_the_tongue_phenomenon#experiences">
        <rdfs:domain rdf:resource="http://www.ontologydesignpatterns.org/ont/dul/DUL.owl#SocialAgent"/>
        <rdfs:range>
            <owl:Class>
                <owl:unionOf rdf:parseType="Collection">
                    <rdf:Description rdf:about="http://www.semanticweb.org/mguen/ontologies/2024/1/CognitiveBiasOntology/tip_of_the_tongue_phenomenon#MemoryBlock"/>
                    <rdf:Description rdf:about="http://www.semanticweb.org/mguen/ontologies/2024/1/CognitiveBiasOntology/tip_of_the_tongue_phenomenon#MemoryRetrieval"/>
                </owl:unionOf>
            </owl:Class>
        </rdfs:range>
        <rdfs:comment>A relationship between a Person and a MemoryPhenomenon they experience.</rdfs:comment>
    </owl:ObjectProperty>
    


    <!-- http://www.semanticweb.org/mguen/ontologies/2024/1/CognitiveBiasOntology/tip_of_the_tongue_phenomenon#lackInformationObject -->

    <owl:ObjectProperty rdf:about="http://www.semanticweb.org/mguen/ontologies/2024/1/CognitiveBiasOntology/tip_of_the_tongue_phenomenon#lackInformationObject">
        <rdfs:domain rdf:resource="http://www.ontologydesignpatterns.org/ont/dul/DUL.owl#SocialAgent"/>
        <rdfs:range rdf:resource="http://krisnadhi.github.io/onto/event.owl#InformationObject"/>
        <rdfs:comment>This property was created for the purpose of negating hasInformationObject. The intent is to make it clear that an unsuccessful recall is such because it lacks the information object it would need to be a successful recall.</rdfs:comment>
    </owl:ObjectProperty>
    


    <!-- http://www.semanticweb.org/mguen/ontologies/2024/1/CognitiveBiasOntology/tip_of_the_tongue_phenomenon#resolvedBy -->

    <owl:ObjectProperty rdf:about="http://www.semanticweb.org/mguen/ontologies/2024/1/CognitiveBiasOntology/tip_of_the_tongue_phenomenon#resolvedBy">
        <rdfs:domain rdf:resource="http://www.semanticweb.org/mguen/ontologies/2024/1/CognitiveBiasOntology/tip_of_the_tongue_phenomenon#MemoryBlock"/>
        <rdfs:range rdf:resource="http://www.semanticweb.org/mguen/ontologies/2024/1/CognitiveBiasOntology/tip_of_the_tongue_phenomenon#MemoryRetrieval"/>
        <rdfs:comment>A relationship between a MemoryBlock and a MemoryRetrieval it is resolved by.</rdfs:comment>
    </owl:ObjectProperty>
    


    <!-- 
    ///////////////////////////////////////////////////////////////////////////////////////
    //
    // Data properties
    //
    ///////////////////////////////////////////////////////////////////////////////////////
     -->

    


    <!-- http://www.semanticweb.org/mguen/ontologies/2024/1/CognitiveBiasOntology/tip_of_the_tongue_phenomenon#isSuccessful -->

    <owl:DatatypeProperty rdf:about="http://www.semanticweb.org/mguen/ontologies/2024/1/CognitiveBiasOntology/tip_of_the_tongue_phenomenon#isSuccessful">
        <rdfs:domain>
            <owl:Class>
                <owl:unionOf rdf:parseType="Collection">
                    <rdf:Description rdf:about="http://etna.istc.cnr.it/framester2/data/framestercore/Memory"/>
                    <rdf:Description rdf:about="http://www.semanticweb.org/mguen/ontologies/2024/1/CognitiveBiasOntology/tip_of_the_tongue_phenomenon#RecallAttempt"/>
                </owl:unionOf>
            </owl:Class>
        </rdfs:domain>
        <rdfs:range rdf:resource="http://www.w3.org/2001/XMLSchema#boolean"/>
        <rdfs:comment>Denotes if the recall attempt is successful or not, resulting in a persistent state of memory block or a state of memory retrieval. By extension denotes if the Memory class, that have a binary meaning as stated in the class description, is more about rememberinbg or forgettin an information.</rdfs:comment>
    </owl:DatatypeProperty>
    


    <!-- 
    ///////////////////////////////////////////////////////////////////////////////////////
    //
    // Classes
    //
    ///////////////////////////////////////////////////////////////////////////////////////
     -->

    


    <!-- http://etna.istc.cnr.it/framester2/data/framestercore/Memory -->

    <owl:Class rdf:about="http://etna.istc.cnr.it/framester2/data/framestercore/Memory">
        <rdfs:comment>This frame is concerned with Cognizers remembering and forgetting mental Content.</rdfs:comment>
    </owl:Class>
    


    <!-- http://krisnadhi.github.io/onto/event.owl#Event -->

    <owl:Class rdf:about="http://krisnadhi.github.io/onto/event.owl#Event">
        <rdfs:comment>Represents any kind of events. An event possesses a spatiotemporal extent, provides at least one participant-role, which is performed by some entity (agents or otherwise), and may be a sub-event of another event. An event may also have additional descriptive information, which is consolidated through an information object</rdfs:comment>
    </owl:Class>
    


    <!-- http://krisnadhi.github.io/onto/event.owl#InformationObject -->

    <owl:Class rdf:about="http://krisnadhi.github.io/onto/event.owl#InformationObject">
        <rdfs:comment>An entity that encapsulates all descriptive or non-defining information of the corresponding event, e.g., names, additional identifiers, textual descriptions, etc. Should normally be aligned to a separate Information Object pattern</rdfs:comment>
        <rdfs:comment>Represents a piece of knowledge or data.</rdfs:comment>
    </owl:Class>
    


    <!-- http://www.ontologydesignpatterns.org/ont/dul/DUL.owl#SocialAgent -->

    <owl:Class rdf:about="http://www.ontologydesignpatterns.org/ont/dul/DUL.owl#SocialAgent">
        <owl:equivalentClass>
            <owl:Restriction>
                <owl:onProperty rdf:resource="http://krisnadhi.github.io/onto/event.owl#hasInformationObject"/>
                <owl:someValuesFrom>
                    <owl:Class>
                        <owl:intersectionOf rdf:parseType="Collection">
                            <rdf:Description rdf:about="http://krisnadhi.github.io/onto/event.owl#InformationObject"/>
                            <owl:Restriction>
                                <owl:onProperty rdf:resource="http://www.semanticweb.org/mguen/ontologies/2024/1/CognitiveBiasOntology/tip_of_the_tongue_phenomenon#attemptsRecall"/>
                                <owl:someValuesFrom>
                                    <owl:Class>
                                        <owl:intersectionOf rdf:parseType="Collection">
                                            <rdf:Description rdf:about="http://www.semanticweb.org/mguen/ontologies/2024/1/CognitiveBiasOntology/tip_of_the_tongue_phenomenon#RecallAttempt"/>
                                            <owl:Restriction>
                                                <owl:onProperty rdf:resource="http://www.semanticweb.org/mguen/ontologies/2024/1/CognitiveBiasOntology/tip_of_the_tongue_phenomenon#isSuccessful"/>
                                                <owl:hasValue rdf:datatype="http://www.w3.org/2001/XMLSchema#boolean">true</owl:hasValue>
                                            </owl:Restriction>
                                        </owl:intersectionOf>
                                    </owl:Class>
                                </owl:someValuesFrom>
                            </owl:Restriction>
                        </owl:intersectionOf>
                    </owl:Class>
                </owl:someValuesFrom>
            </owl:Restriction>
        </owl:equivalentClass>
        <owl:equivalentClass>
            <owl:Restriction>
                <owl:onProperty rdf:resource="http://www.semanticweb.org/mguen/ontologies/2024/1/CognitiveBiasOntology/tip_of_the_tongue_phenomenon#experiences"/>
                <owl:someValuesFrom>
                    <owl:Class>
                        <owl:intersectionOf rdf:parseType="Collection">
                            <rdf:Description rdf:about="http://www.semanticweb.org/mguen/ontologies/2024/1/CognitiveBiasOntology/tip_of_the_tongue_phenomenon#MemoryBlock"/>
                            <owl:Restriction>
                                <owl:onProperty rdf:resource="http://www.semanticweb.org/mguen/ontologies/2024/1/CognitiveBiasOntology/tip_of_the_tongue_phenomenon#attemptsRecall"/>
                                <owl:someValuesFrom>
                                    <owl:Class>
                                        <owl:intersectionOf rdf:parseType="Collection">
                                            <rdf:Description rdf:about="http://www.semanticweb.org/mguen/ontologies/2024/1/CognitiveBiasOntology/tip_of_the_tongue_phenomenon#RecallAttempt"/>
                                            <owl:Restriction>
                                                <owl:onProperty rdf:resource="http://www.semanticweb.org/mguen/ontologies/2024/1/CognitiveBiasOntology/tip_of_the_tongue_phenomenon#isSuccessful"/>
                                                <owl:hasValue rdf:datatype="http://www.w3.org/2001/XMLSchema#boolean">false</owl:hasValue>
                                            </owl:Restriction>
                                        </owl:intersectionOf>
                                    </owl:Class>
                                </owl:someValuesFrom>
                            </owl:Restriction>
                        </owl:intersectionOf>
                    </owl:Class>
                </owl:someValuesFrom>
            </owl:Restriction>
        </owl:equivalentClass>
        <owl:equivalentClass>
            <owl:Restriction>
                <owl:onProperty rdf:resource="http://www.semanticweb.org/mguen/ontologies/2024/1/CognitiveBiasOntology/tip_of_the_tongue_phenomenon#experiences"/>
                <owl:someValuesFrom>
                    <owl:Class>
                        <owl:intersectionOf rdf:parseType="Collection">
                            <rdf:Description rdf:about="http://www.semanticweb.org/mguen/ontologies/2024/1/CognitiveBiasOntology/tip_of_the_tongue_phenomenon#MemoryRetrieval"/>
                            <owl:Restriction>
                                <owl:onProperty rdf:resource="http://www.semanticweb.org/mguen/ontologies/2024/1/CognitiveBiasOntology/tip_of_the_tongue_phenomenon#attemptsRecall"/>
                                <owl:someValuesFrom>
                                    <owl:Class>
                                        <owl:intersectionOf rdf:parseType="Collection">
                                            <rdf:Description rdf:about="http://www.semanticweb.org/mguen/ontologies/2024/1/CognitiveBiasOntology/tip_of_the_tongue_phenomenon#RecallAttempt"/>
                                            <owl:Restriction>
                                                <owl:onProperty rdf:resource="http://www.semanticweb.org/mguen/ontologies/2024/1/CognitiveBiasOntology/tip_of_the_tongue_phenomenon#isSuccessful"/>
                                                <owl:hasValue rdf:datatype="http://www.w3.org/2001/XMLSchema#boolean">true</owl:hasValue>
                                            </owl:Restriction>
                                        </owl:intersectionOf>
                                    </owl:Class>
                                </owl:someValuesFrom>
                            </owl:Restriction>
                        </owl:intersectionOf>
                    </owl:Class>
                </owl:someValuesFrom>
            </owl:Restriction>
        </owl:equivalentClass>
        <owl:equivalentClass>
            <owl:Restriction>
                <owl:onProperty rdf:resource="http://www.semanticweb.org/mguen/ontologies/2024/1/CognitiveBiasOntology/tip_of_the_tongue_phenomenon#lackInformationObject"/>
                <owl:someValuesFrom>
                    <owl:Class>
                        <owl:intersectionOf rdf:parseType="Collection">
                            <rdf:Description rdf:about="http://krisnadhi.github.io/onto/event.owl#InformationObject"/>
                            <owl:Restriction>
                                <owl:onProperty rdf:resource="http://www.semanticweb.org/mguen/ontologies/2024/1/CognitiveBiasOntology/tip_of_the_tongue_phenomenon#attemptsRecall"/>
                                <owl:someValuesFrom>
                                    <owl:Class>
                                        <owl:intersectionOf rdf:parseType="Collection">
                                            <rdf:Description rdf:about="http://www.semanticweb.org/mguen/ontologies/2024/1/CognitiveBiasOntology/tip_of_the_tongue_phenomenon#RecallAttempt"/>
                                            <owl:Restriction>
                                                <owl:onProperty rdf:resource="http://www.semanticweb.org/mguen/ontologies/2024/1/CognitiveBiasOntology/tip_of_the_tongue_phenomenon#isSuccessful"/>
                                                <owl:hasValue rdf:datatype="http://www.w3.org/2001/XMLSchema#boolean">true</owl:hasValue>
                                            </owl:Restriction>
                                        </owl:intersectionOf>
                                    </owl:Class>
                                </owl:someValuesFrom>
                            </owl:Restriction>
                        </owl:intersectionOf>
                    </owl:Class>
                </owl:someValuesFrom>
            </owl:Restriction>
        </owl:equivalentClass>
        <rdfs:comment>(owl:Class) Any individual whose existence is granted simply by its social communicability and capability of action (through some PhysicalAgent)</rdfs:comment>
        <rdfs:comment>A SocialAgent experiences a MemoryBlock if the RecallAttempt is unsuccessful (i.e., isSuccessful value is false).
A SocialAgent experiences a MemoryRetrieval if the RecallAttempt is successful (i.e., isSuccessful value is true).
A SocialAgent has an InformationObject if the RecallAttempt is successful (i.e., isSuccessful value is true).
A SocialAgent lacks an InformationObject if the RecallAttempt is successful (i.e., isSuccessful value is true).</rdfs:comment>
        <rdfs:comment>Represents an individual human being.</rdfs:comment>
    </owl:Class>
    


    <!-- http://www.semanticweb.org/mguen/ontologies/2024/1/CognitiveBiasOntology/tip_of_the_tongue_phenomenon#MemoryBlock -->

    <owl:Class rdf:about="http://www.semanticweb.org/mguen/ontologies/2024/1/CognitiveBiasOntology/tip_of_the_tongue_phenomenon#MemoryBlock">
        <rdfs:subClassOf>
            <owl:Class>
                <owl:intersectionOf rdf:parseType="Collection">
                    <rdf:Description rdf:about="http://etna.istc.cnr.it/framester2/data/framestercore/Memory"/>
                    <owl:Restriction>
                        <owl:onProperty rdf:resource="http://www.semanticweb.org/mguen/ontologies/2024/1/CognitiveBiasOntology/tip_of_the_tongue_phenomenon#isSuccessful"/>
                        <owl:hasValue rdf:datatype="http://www.w3.org/2001/XMLSchema#boolean">false</owl:hasValue>
                    </owl:Restriction>
                </owl:intersectionOf>
            </owl:Class>
        </rdfs:subClassOf>
        <rdfs:comment>Represents a block or obstacle in the process of recalling information.</rdfs:comment>
    </owl:Class>
    


    <!-- http://www.semanticweb.org/mguen/ontologies/2024/1/CognitiveBiasOntology/tip_of_the_tongue_phenomenon#MemoryRetrieval -->

    <owl:Class rdf:about="http://www.semanticweb.org/mguen/ontologies/2024/1/CognitiveBiasOntology/tip_of_the_tongue_phenomenon#MemoryRetrieval">
        <rdfs:subClassOf>
            <owl:Class>
                <owl:intersectionOf rdf:parseType="Collection">
                    <rdf:Description rdf:about="http://etna.istc.cnr.it/framester2/data/framestercore/Memory"/>
                    <owl:Restriction>
                        <owl:onProperty rdf:resource="http://www.semanticweb.org/mguen/ontologies/2024/1/CognitiveBiasOntology/tip_of_the_tongue_phenomenon#isSuccessful"/>
                        <owl:hasValue rdf:datatype="http://www.w3.org/2001/XMLSchema#boolean">true</owl:hasValue>
                    </owl:Restriction>
                </owl:intersectionOf>
            </owl:Class>
        </rdfs:subClassOf>
        <rdfs:comment>Represents the process of retrieving information from memory.</rdfs:comment>
    </owl:Class>
    


    <!-- http://www.semanticweb.org/mguen/ontologies/2024/1/CognitiveBiasOntology/tip_of_the_tongue_phenomenon#RecallAttempt -->

    <owl:Class rdf:about="http://www.semanticweb.org/mguen/ontologies/2024/1/CognitiveBiasOntology/tip_of_the_tongue_phenomenon#RecallAttempt">
        <owl:equivalentClass>
            <owl:Restriction>
                <owl:onProperty rdf:resource="http://www.ontology.se/odp/content/owl/Action.owl#has_consequence"/>
                <owl:someValuesFrom>
                    <owl:Class>
                        <owl:intersectionOf rdf:parseType="Collection">
                            <rdf:Description rdf:about="http://www.semanticweb.org/mguen/ontologies/2024/1/CognitiveBiasOntology/tip_of_the_tongue_phenomenon#MemoryBlock"/>
                            <owl:Restriction>
                                <owl:onProperty rdf:resource="http://www.semanticweb.org/mguen/ontologies/2024/1/CognitiveBiasOntology/tip_of_the_tongue_phenomenon#isSuccessful"/>
                                <owl:hasValue rdf:datatype="http://www.w3.org/2001/XMLSchema#boolean">false</owl:hasValue>
                            </owl:Restriction>
                        </owl:intersectionOf>
                    </owl:Class>
                </owl:someValuesFrom>
            </owl:Restriction>
        </owl:equivalentClass>
        <owl:equivalentClass>
            <owl:Restriction>
                <owl:onProperty rdf:resource="http://www.ontology.se/odp/content/owl/Action.owl#has_consequence"/>
                <owl:someValuesFrom>
                    <owl:Class>
                        <owl:intersectionOf rdf:parseType="Collection">
                            <rdf:Description rdf:about="http://www.semanticweb.org/mguen/ontologies/2024/1/CognitiveBiasOntology/tip_of_the_tongue_phenomenon#MemoryRetrieval"/>
                            <owl:Restriction>
                                <owl:onProperty rdf:resource="http://www.semanticweb.org/mguen/ontologies/2024/1/CognitiveBiasOntology/tip_of_the_tongue_phenomenon#isSuccessful"/>
                                <owl:hasValue rdf:datatype="http://www.w3.org/2001/XMLSchema#boolean">true</owl:hasValue>
                            </owl:Restriction>
                        </owl:intersectionOf>
                    </owl:Class>
                </owl:someValuesFrom>
            </owl:Restriction>
        </owl:equivalentClass>
        <rdfs:subClassOf rdf:resource="http://krisnadhi.github.io/onto/event.owl#Event"/>
        <rdfs:comment>A RecallAttempt has a consequence of MemoryBlock if the isSuccessful value is false, and it has a consequence of MemoryRetrieval if the isSuccessful value is true.</rdfs:comment>
        <rdfs:comment>Represents an attempt made by a person to recall information.</rdfs:comment>
    </owl:Class>
    


    <!-- 
    ///////////////////////////////////////////////////////////////////////////////////////
    //
    // Individuals
    //
    ///////////////////////////////////////////////////////////////////////////////////////
     -->

    


    <!-- http://www.semanticweb.org/mguen/ontologies/2024/1/CognitiveBiasOntology/tip_of_the_tongue_phenomenon#Amanda -->

    <owl:NamedIndividual rdf:about="http://www.semanticweb.org/mguen/ontologies/2024/1/CognitiveBiasOntology/tip_of_the_tongue_phenomenon#Amanda">
        <rdf:type rdf:resource="http://www.ontologydesignpatterns.org/ont/dul/DUL.owl#SocialAgent"/>
    </owl:NamedIndividual>
    


    <!-- http://www.semanticweb.org/mguen/ontologies/2024/1/CognitiveBiasOntology/tip_of_the_tongue_phenomenon#DressColor -->

    <owl:NamedIndividual rdf:about="http://www.semanticweb.org/mguen/ontologies/2024/1/CognitiveBiasOntology/tip_of_the_tongue_phenomenon#DressColor">
        <rdf:type rdf:resource="http://krisnadhi.github.io/onto/event.owl#InformationObject"/>
    </owl:NamedIndividual>
    


    <!-- http://www.semanticweb.org/mguen/ontologies/2024/1/CognitiveBiasOntology/tip_of_the_tongue_phenomenon#Emily -->

    <owl:NamedIndividual rdf:about="http://www.semanticweb.org/mguen/ontologies/2024/1/CognitiveBiasOntology/tip_of_the_tongue_phenomenon#Emily">
        <rdf:type rdf:resource="http://www.ontologydesignpatterns.org/ont/dul/DUL.owl#SocialAgent"/>
        <event:hasInformationObject rdf:resource="http://www.semanticweb.org/mguen/ontologies/2024/1/CognitiveBiasOntology/tip_of_the_tongue_phenomenon#DressColor"/>
        <event:hasInformationObject rdf:resource="http://www.semanticweb.org/mguen/ontologies/2024/1/CognitiveBiasOntology/tip_of_the_tongue_phenomenon#Face"/>
        <event:hasInformationObject rdf:resource="http://www.semanticweb.org/mguen/ontologies/2024/1/CognitiveBiasOntology/tip_of_the_tongue_phenomenon#ProjectDetails"/>
        <attemptsRecall rdf:resource="http://www.semanticweb.org/mguen/ontologies/2024/1/CognitiveBiasOntology/tip_of_the_tongue_phenomenon#FirstRecallAttempt"/>
        <experiences rdf:resource="http://www.semanticweb.org/mguen/ontologies/2024/1/CognitiveBiasOntology/tip_of_the_tongue_phenomenon#MemoryBlockIstance"/>
        <experiences rdf:resource="http://www.semanticweb.org/mguen/ontologies/2024/1/CognitiveBiasOntology/tip_of_the_tongue_phenomenon#MemoryRetrievalIstance"/>
        <lackInformationObject rdf:resource="http://www.semanticweb.org/mguen/ontologies/2024/1/CognitiveBiasOntology/tip_of_the_tongue_phenomenon#Name"/>
    </owl:NamedIndividual>
    


    <!-- http://www.semanticweb.org/mguen/ontologies/2024/1/CognitiveBiasOntology/tip_of_the_tongue_phenomenon#Face -->

    <owl:NamedIndividual rdf:about="http://www.semanticweb.org/mguen/ontologies/2024/1/CognitiveBiasOntology/tip_of_the_tongue_phenomenon#Face">
        <rdf:type rdf:resource="http://krisnadhi.github.io/onto/event.owl#InformationObject"/>
    </owl:NamedIndividual>
    


    <!-- http://www.semanticweb.org/mguen/ontologies/2024/1/CognitiveBiasOntology/tip_of_the_tongue_phenomenon#FirstRecallAttempt -->

    <owl:NamedIndividual rdf:about="http://www.semanticweb.org/mguen/ontologies/2024/1/CognitiveBiasOntology/tip_of_the_tongue_phenomenon#FirstRecallAttempt">
        <rdf:type rdf:resource="http://www.semanticweb.org/mguen/ontologies/2024/1/CognitiveBiasOntology/tip_of_the_tongue_phenomenon#RecallAttempt"/>
        <Action:has_consequence rdf:resource="http://www.semanticweb.org/mguen/ontologies/2024/1/CognitiveBiasOntology/tip_of_the_tongue_phenomenon#MemoryBlockIstance"/>
        <isSuccessful rdf:datatype="http://www.w3.org/2001/XMLSchema#boolean">false</isSuccessful>
    </owl:NamedIndividual>
    


    <!-- http://www.semanticweb.org/mguen/ontologies/2024/1/CognitiveBiasOntology/tip_of_the_tongue_phenomenon#MemoryBlockIstance -->

    <owl:NamedIndividual rdf:about="http://www.semanticweb.org/mguen/ontologies/2024/1/CognitiveBiasOntology/tip_of_the_tongue_phenomenon#MemoryBlockIstance">
        <rdf:type rdf:resource="http://www.semanticweb.org/mguen/ontologies/2024/1/CognitiveBiasOntology/tip_of_the_tongue_phenomenon#MemoryBlock"/>
        <resolvedBy rdf:resource="http://www.semanticweb.org/mguen/ontologies/2024/1/CognitiveBiasOntology/tip_of_the_tongue_phenomenon#MemoryRetrievalIstance"/>
    </owl:NamedIndividual>
    


    <!-- http://www.semanticweb.org/mguen/ontologies/2024/1/CognitiveBiasOntology/tip_of_the_tongue_phenomenon#MemoryRetrievalIstance -->

    <owl:NamedIndividual rdf:about="http://www.semanticweb.org/mguen/ontologies/2024/1/CognitiveBiasOntology/tip_of_the_tongue_phenomenon#MemoryRetrievalIstance">
        <rdf:type rdf:resource="http://www.semanticweb.org/mguen/ontologies/2024/1/CognitiveBiasOntology/tip_of_the_tongue_phenomenon#MemoryRetrieval"/>
    </owl:NamedIndividual>
    


    <!-- http://www.semanticweb.org/mguen/ontologies/2024/1/CognitiveBiasOntology/tip_of_the_tongue_phenomenon#Name -->

    <owl:NamedIndividual rdf:about="http://www.semanticweb.org/mguen/ontologies/2024/1/CognitiveBiasOntology/tip_of_the_tongue_phenomenon#Name">
        <rdf:type rdf:resource="http://krisnadhi.github.io/onto/event.owl#InformationObject"/>
    </owl:NamedIndividual>
    


    <!-- http://www.semanticweb.org/mguen/ontologies/2024/1/CognitiveBiasOntology/tip_of_the_tongue_phenomenon#ProjectDetails -->

    <owl:NamedIndividual rdf:about="http://www.semanticweb.org/mguen/ontologies/2024/1/CognitiveBiasOntology/tip_of_the_tongue_phenomenon#ProjectDetails">
        <rdf:type rdf:resource="http://krisnadhi.github.io/onto/event.owl#InformationObject"/>
    </owl:NamedIndividual>
    


    <!-- http://www.semanticweb.org/mguen/ontologies/2024/1/CognitiveBiasOntology/tip_of_the_tongue_phenomenon#SecondRecallAttempt -->

    <owl:NamedIndividual rdf:about="http://www.semanticweb.org/mguen/ontologies/2024/1/CognitiveBiasOntology/tip_of_the_tongue_phenomenon#SecondRecallAttempt">
        <rdf:type rdf:resource="http://www.semanticweb.org/mguen/ontologies/2024/1/CognitiveBiasOntology/tip_of_the_tongue_phenomenon#RecallAttempt"/>
        <Action:has_consequence rdf:resource="http://www.semanticweb.org/mguen/ontologies/2024/1/CognitiveBiasOntology/tip_of_the_tongue_phenomenon#MemoryRetrievalIstance"/>
    </owl:NamedIndividual>
</rdf:RDF>



<!-- Generated by the OWL API (version 4.5.25.2023-02-15T19:15:49Z) https://github.com/owlcs/owlapi -->

